proofs/fstar/extraction/Polytune.Faand.fst
@@ -3,17 +3,6 @@ module Polytune.Faand
 open Core
 open FStar.Mul
 
-let _ =
-  (* This module has implicit dependencies, here we make them explicit. *)
-  (* The implicit dependencies arise from typeclasses instances. *)
-  let open Polytune.Channel in
-  let open Polytune.Data_types in
-  let open Serde.De in
-  let open Serde.De.Impls in
-  let open Serde.Ser in
-  let open Serde.Ser.Impls in
-  ()
-
 /// Errors occurring during preprocessing.
 type t_Error =
   | Error_ChannelErr : Polytune.Channel.t_Error -> t_Error
@@ -33,47 +22,8 @@ type t_Error =
   | Error_BeaverWrongMAC : t_Error
   | Error_InvalidHashLength : t_Error
 
-/// Converts a `channel::Error` into a custom `Error` type.
-[@@ FStar.Tactics.Typeclasses.tcinstance]
-let impl: Core.Convert.t_From t_Error Polytune.Channel.t_Error =
-  {
-    f_from_pre = (fun (e: Polytune.Channel.t_Error) -> true);
-    f_from_post = (fun (e: Polytune.Channel.t_Error) (out: t_Error) -> true);
-    f_from = fun (e: Polytune.Channel.t_Error) -> Error_ChannelErr e <: t_Error
-  }
-
 /// Represents a cryptographic commitment as a fixed-size 32-byte array (a BLAKE3 hash).
 type t_Commitment = | Commitment : t_Array u8 (mk_usize 32) -> t_Commitment
-
-[@@ FStar.Tactics.Typeclasses.tcinstance]
-assume
-val impl_2': Core.Fmt.t_Debug t_Commitment
-
-unfold
-let impl_2 = impl_2'
-
-let impl_3: Core.Clone.t_Clone t_Commitment = { f_clone = (fun x -> x) }
-
-[@@ FStar.Tactics.Typeclasses.tcinstance]
-assume
-val e___impl': Serde.Ser.t_Serialize t_Commitment
-
-unfold
-let e___impl = e___impl'
-
-[@@ FStar.Tactics.Typeclasses.tcinstance]
-assume
-val e_ee_1__impl': Serde.De.t_Deserialize t_Commitment
-
-unfold
-let e_ee_1__impl = e_ee_1__impl'
-
-[@@ FStar.Tactics.Typeclasses.tcinstance]
-assume
-val impl_6': Core.Cmp.t_PartialEq t_Commitment t_Commitment
-
-unfold
-let impl_6 = impl_6'
 
 /// Commits to a value using the BLAKE3 cryptographic hash function.
 /// This is not a general-purpose commitment scheme, the input value is assumed to have high entropy.
@@ -89,204 +39,191 @@ let open_commitment (commitment: t_Commitment) (value: t_Slice u8) : bool =
   (Blake3.impl_Hash__as_bytes (Blake3.hash value <: Blake3.t_Hash) <: t_Array u8 (mk_usize 32)) =.
   commitment._0
 
-/// Implements broadcast with abort based on Goldwasser and Lindell\'s protocol
-/// for all parties at once, where each party sends its vector to all others.
-/// The function returns the vector received and verified by broadcast.
-assume
-val broadcast':
-    #v_T: Type0 ->
-    #iimpl_951670863_: Type0 ->
-    {| i2: Core.Clone.t_Clone v_T |} ->
-    {| i3: Serde.Ser.t_Serialize v_T |} ->
-    {| i4: Serde.De.t_DeserializeOwned v_T |} ->
-    {| i5: Core.Fmt.t_Debug v_T |} ->
-    {| i6: Core.Cmp.t_PartialEq v_T v_T |} ->
-    {| i7: Polytune.Channel.t_Channel iimpl_951670863_ |} ->
-    channel: iimpl_951670863_ ->
-    i: usize ->
-    n: usize ->
-    phase: string ->
-    vec: t_Slice v_T ->
-    len: usize
-  -> (iimpl_951670863_ &
-      Core.Result.t_Result
-        (Alloc.Vec.t_Vec (Alloc.Vec.t_Vec v_T Alloc.Alloc.t_Global) Alloc.Alloc.t_Global) t_Error)
-
-unfold
-let broadcast
-      (#v_T #iimpl_951670863_: Type0)
-      (#[FStar.Tactics.Typeclasses.tcresolve ()] i2: Core.Clone.t_Clone v_T)
-      (#[FStar.Tactics.Typeclasses.tcresolve ()] i3: Serde.Ser.t_Serialize v_T)
-      (#[FStar.Tactics.Typeclasses.tcresolve ()] i4: Serde.De.t_DeserializeOwned v_T)
-      (#[FStar.Tactics.Typeclasses.tcresolve ()] i5: Core.Fmt.t_Debug v_T)
-      (#[FStar.Tactics.Typeclasses.tcresolve ()] i6: Core.Cmp.t_PartialEq v_T v_T)
-      (#[FStar.Tactics.Typeclasses.tcresolve ()] i7: Polytune.Channel.t_Channel iimpl_951670863_)
-     = broadcast' #v_T #iimpl_951670863_ #i2 #i3 #i4 #i5 #i6 #i7
-
-/// Implements same broadcast with abort as broadcast, but only the first element of the tuple in
-/// the vector is broadcasted, the second element is simply sent to all parties.
-assume
-val broadcast_first_send_second':
-    #v_T: Type0 ->
-    #v_S: Type0 ->
-    #iimpl_951670863_: Type0 ->
-    {| i3: Core.Clone.t_Clone v_T |} ->
-    {| i4: Serde.Ser.t_Serialize v_T |} ->
-    {| i5: Serde.De.t_DeserializeOwned v_T |} ->
-    {| i6: Core.Fmt.t_Debug v_T |} ->
-    {| i7: Core.Cmp.t_PartialEq v_T v_T |} ->
-    {| i8: Core.Clone.t_Clone v_S |} ->
-    {| i9: Serde.Ser.t_Serialize v_S |} ->
-    {| i10: Serde.De.t_DeserializeOwned v_S |} ->
-    {| i11: Core.Fmt.t_Debug v_S |} ->
-    {| i12: Core.Cmp.t_PartialEq v_S v_S |} ->
-    {| i13: Polytune.Channel.t_Channel iimpl_951670863_ |} ->
-    channel: iimpl_951670863_ ->
-    i: usize ->
-    n: usize ->
-    phase: string ->
-    vec: t_Slice (Alloc.Vec.t_Vec (v_T & v_S) Alloc.Alloc.t_Global) ->
-    len: usize
-  -> (iimpl_951670863_ &
-      Core.Result.t_Result
-        (Alloc.Vec.t_Vec (Alloc.Vec.t_Vec (v_T & v_S) Alloc.Alloc.t_Global) Alloc.Alloc.t_Global)
-        t_Error)
-
-unfold
-let broadcast_first_send_second
-      (#v_T #v_S #iimpl_951670863_: Type0)
-      (#[FStar.Tactics.Typeclasses.tcresolve ()] i3: Core.Clone.t_Clone v_T)
-      (#[FStar.Tactics.Typeclasses.tcresolve ()] i4: Serde.Ser.t_Serialize v_T)
-      (#[FStar.Tactics.Typeclasses.tcresolve ()] i5: Serde.De.t_DeserializeOwned v_T)
-      (#[FStar.Tactics.Typeclasses.tcresolve ()] i6: Core.Fmt.t_Debug v_T)
-      (#[FStar.Tactics.Typeclasses.tcresolve ()] i7: Core.Cmp.t_PartialEq v_T v_T)
-      (#[FStar.Tactics.Typeclasses.tcresolve ()] i8: Core.Clone.t_Clone v_S)
-      (#[FStar.Tactics.Typeclasses.tcresolve ()] i9: Serde.Ser.t_Serialize v_S)
-      (#[FStar.Tactics.Typeclasses.tcresolve ()] i10: Serde.De.t_DeserializeOwned v_S)
-      (#[FStar.Tactics.Typeclasses.tcresolve ()] i11: Core.Fmt.t_Debug v_S)
-      (#[FStar.Tactics.Typeclasses.tcresolve ()] i12: Core.Cmp.t_PartialEq v_S v_S)
-      (#[FStar.Tactics.Typeclasses.tcresolve ()] i13: Polytune.Channel.t_Channel iimpl_951670863_)
-     =
-  broadcast_first_send_second' #v_T #v_S #iimpl_951670863_ #i3 #i4 #i5 #i6 #i7 #i8 #i9 #i10 #i11
-    #i12 #i13
-
 assume
 val random_bool': Prims.unit -> bool
 
 unfold
 let random_bool = random_bool'
 
-/// Protocol Pi_HaAND that performs F_HaAND from the paper
-/// [Global-Scale Secure Multiparty Computation](https://dl.acm.org/doi/pdf/10.1145/3133956.3133979).
-/// This protocol computes the half-authenticated AND of two bit strings.
-/// The XOR of xiyj values are generated obliviously, which is half of the z value in an
-/// authenticated share, i.e., a half-authenticated share.
-let fhaand
-      (#iimpl_951670863_: Type0)
-      (#[FStar.Tactics.Typeclasses.tcresolve ()] i1: Polytune.Channel.t_Channel iimpl_951670863_)
-      (channel: iimpl_951670863_)
+let fhaand_1_
       (delta: Polytune.Data_types.t_Delta)
       (i n l: usize)
       (xshares: t_Slice Polytune.Data_types.t_Share)
       (yi: Alloc.Vec.t_Vec bool Alloc.Alloc.t_Global)
-    : (iimpl_951670863_ & Core.Result.t_Result (Alloc.Vec.t_Vec bool Alloc.Alloc.t_Global) t_Error) =
-  if (Core.Slice.impl__len #Polytune.Data_types.t_Share xshares <: usize) <>. l
-  then
-    channel,
-    (Core.Result.Result_Err (Error_InvalidLength <: t_Error)
-      <:
-      Core.Result.t_Result (Alloc.Vec.t_Vec bool Alloc.Alloc.t_Global) t_Error)
-    <:
-    (iimpl_951670863_ & Core.Result.t_Result (Alloc.Vec.t_Vec bool Alloc.Alloc.t_Global) t_Error)
-  else
-    let vi:Alloc.Vec.t_Vec bool Alloc.Alloc.t_Global = Alloc.Vec.from_elem #bool false l in
-    let h0h1:Alloc.Vec.t_Vec (bool & bool) Alloc.Alloc.t_Global =
-      Alloc.Vec.from_elem #(bool & bool) (false, false <: (bool & bool)) l
-    in
-    match
-      Rust_primitives.Hax.Folds.fold_range_return (mk_usize 0)
-        n
-        (fun temp_0_ temp_1_ ->
-            let channel, h0h1, vi:(iimpl_951670863_ &
-              Alloc.Vec.t_Vec (bool & bool) Alloc.Alloc.t_Global &
-              Alloc.Vec.t_Vec bool Alloc.Alloc.t_Global) =
-              temp_0_
-            in
-            let _:usize = temp_1_ in
-            true)
-        (channel, h0h1, vi
-          <:
-          (iimpl_951670863_ & Alloc.Vec.t_Vec (bool & bool) Alloc.Alloc.t_Global &
-            Alloc.Vec.t_Vec bool Alloc.Alloc.t_Global))
-        (fun temp_0_ j ->
-            let channel, h0h1, vi:(iimpl_951670863_ &
-              Alloc.Vec.t_Vec (bool & bool) Alloc.Alloc.t_Global &
-              Alloc.Vec.t_Vec bool Alloc.Alloc.t_Global) =
-              temp_0_
-            in
-            let j:usize = j in
-            if j =. i <: bool
-            then
-              Core.Ops.Control_flow.ControlFlow_Continue
-              (channel, h0h1, vi
+    : Prims.Pure
+      (Alloc.Vec.t_Vec bool Alloc.Alloc.t_Global &
+        Alloc.Vec.t_Vec (Alloc.Vec.t_Vec (bool & bool) Alloc.Alloc.t_Global) Alloc.Alloc.t_Global)
+      (requires
+        b2t ((Alloc.Vec.impl_1__len #bool #Alloc.Alloc.t_Global yi <: usize) >=. l <: bool) /\
+        b2t ((Core.Slice.impl__len #Polytune.Data_types.t_Share xshares <: usize) >=. l <: bool) /\
+        (forall (ll: usize).
+            b2t
+            ((mk_usize 0 <=. ll <: bool) && (ll <. l <: bool) &&
+              ((Core.Slice.impl__len #Polytune.Data_types.t_Share xshares <: usize) >=. l <: bool)) ==>
+            b2t
+            ((Alloc.Vec.impl_1__len #(Polytune.Data_types.t_Mac & Polytune.Data_types.t_Key)
+                  #Alloc.Alloc.t_Global
+                  (xshares.[ ll ] <: Polytune.Data_types.t_Share).Polytune.Data_types._1
+                    .Polytune.Data_types._0
                 <:
-                (iimpl_951670863_ & Alloc.Vec.t_Vec (bool & bool) Alloc.Alloc.t_Global &
-                  Alloc.Vec.t_Vec bool Alloc.Alloc.t_Global))
+                usize) >=.
+              n
               <:
-              Core.Ops.Control_flow.t_ControlFlow
-                (Core.Ops.Control_flow.t_ControlFlow
-                    (iimpl_951670863_ &
-                      Core.Result.t_Result (Alloc.Vec.t_Vec bool Alloc.Alloc.t_Global) t_Error)
-                    (Prims.unit &
-                      (iimpl_951670863_ & Alloc.Vec.t_Vec (bool & bool) Alloc.Alloc.t_Global &
-                        Alloc.Vec.t_Vec bool Alloc.Alloc.t_Global)))
-                (iimpl_951670863_ & Alloc.Vec.t_Vec (bool & bool) Alloc.Alloc.t_Global &
-                  Alloc.Vec.t_Vec bool Alloc.Alloc.t_Global)
-            else
-              let h0h1, vi:(Alloc.Vec.t_Vec (bool & bool) Alloc.Alloc.t_Global &
-                Alloc.Vec.t_Vec bool Alloc.Alloc.t_Global) =
-                Rust_primitives.Hax.Folds.fold_range (mk_usize 0)
-                  l
-                  (fun temp_0_ temp_1_ ->
-                      let h0h1, vi:(Alloc.Vec.t_Vec (bool & bool) Alloc.Alloc.t_Global &
-                        Alloc.Vec.t_Vec bool Alloc.Alloc.t_Global) =
-                        temp_0_
-                      in
-                      let _:usize = temp_1_ in
-                      true)
-                  (h0h1, vi
+              bool)))
+      (fun _ -> Prims.l_True) =
+  let vi:Alloc.Vec.t_Vec bool Alloc.Alloc.t_Global = Alloc.Vec.from_elem #bool false l in
+  let h0h1:Alloc.Vec.t_Vec (Alloc.Vec.t_Vec (bool & bool) Alloc.Alloc.t_Global) Alloc.Alloc.t_Global
+  =
+    Alloc.Vec.from_elem #(Alloc.Vec.t_Vec (bool & bool) Alloc.Alloc.t_Global)
+      (Alloc.Vec.from_elem #(bool & bool) (false, false <: (bool & bool)) l
+        <:
+        Alloc.Vec.t_Vec (bool & bool) Alloc.Alloc.t_Global)
+      n
+  in
+  let h0h1, vi:(Alloc.Vec.t_Vec (Alloc.Vec.t_Vec (bool & bool) Alloc.Alloc.t_Global)
+      Alloc.Alloc.t_Global &
+    Alloc.Vec.t_Vec bool Alloc.Alloc.t_Global) =
+    Rust_primitives.Hax.Folds.fold_range (mk_usize 0)
+      n
+      (fun temp_0_ temp_1_ ->
+          let h0h1, vi:(Alloc.Vec.t_Vec (Alloc.Vec.t_Vec (bool & bool) Alloc.Alloc.t_Global)
+              Alloc.Alloc.t_Global &
+            Alloc.Vec.t_Vec bool Alloc.Alloc.t_Global) =
+            temp_0_
+          in
+          let _:usize = temp_1_ in
+          b2t ((Alloc.Vec.impl_1__len #bool #Alloc.Alloc.t_Global vi <: usize) =. l <: bool) /\
+          b2t
+          ((Alloc.Vec.impl_1__len #(Alloc.Vec.t_Vec (bool & bool) Alloc.Alloc.t_Global)
+                #Alloc.Alloc.t_Global
+                h0h1
+              <:
+              usize) =.
+            n
+            <:
+            bool) /\
+          (forall (j: usize).
+              b2t
+              ((mk_usize 0 <=. j <: bool) && (j <. n <: bool) &&
+                ((Alloc.Vec.impl_1__len #(Alloc.Vec.t_Vec (bool & bool) Alloc.Alloc.t_Global)
+                      #Alloc.Alloc.t_Global
+                      h0h1
                     <:
-                    (Alloc.Vec.t_Vec (bool & bool) Alloc.Alloc.t_Global &
-                      Alloc.Vec.t_Vec bool Alloc.Alloc.t_Global))
-                  (fun temp_0_ ll ->
-                      let h0h1, vi:(Alloc.Vec.t_Vec (bool & bool) Alloc.Alloc.t_Global &
-                        Alloc.Vec.t_Vec bool Alloc.Alloc.t_Global) =
-                        temp_0_
-                      in
-                      let ll:usize = ll in
-                      let (sj: bool):bool = random_bool () in
-                      let _, kixj:(Polytune.Data_types.t_Mac & Polytune.Data_types.t_Key) =
-                        (xshares.[ ll ] <: Polytune.Data_types.t_Share).Polytune.Data_types._1
-                          .Polytune.Data_types._0.[ j ]
-                      in
-                      let hash_kixj:Blake3.t_Hash =
-                        Blake3.hash (Core.Num.impl_u128__to_le_bytes kixj.Polytune.Data_types._0
+                    usize) =.
+                  n
+                  <:
+                  bool)) ==>
+              b2t
+              ((Alloc.Vec.impl_1__len #(bool & bool)
+                    #Alloc.Alloc.t_Global
+                    (h0h1.[ j ] <: Alloc.Vec.t_Vec (bool & bool) Alloc.Alloc.t_Global)
+                  <:
+                  usize) =.
+                l
+                <:
+                bool)))
+      (h0h1, vi
+        <:
+        (Alloc.Vec.t_Vec (Alloc.Vec.t_Vec (bool & bool) Alloc.Alloc.t_Global) Alloc.Alloc.t_Global &
+          Alloc.Vec.t_Vec bool Alloc.Alloc.t_Global))
+      (fun temp_0_ j ->
+          let h0h1, vi:(Alloc.Vec.t_Vec (Alloc.Vec.t_Vec (bool & bool) Alloc.Alloc.t_Global)
+              Alloc.Alloc.t_Global &
+            Alloc.Vec.t_Vec bool Alloc.Alloc.t_Global) =
+            temp_0_
+          in
+          let j:usize = j in
+          if j =. i <: bool
+          then
+            h0h1, vi
+            <:
+            (Alloc.Vec.t_Vec (Alloc.Vec.t_Vec (bool & bool) Alloc.Alloc.t_Global)
+                Alloc.Alloc.t_Global &
+              Alloc.Vec.t_Vec bool Alloc.Alloc.t_Global)
+          else
+            Rust_primitives.Hax.Folds.fold_range (mk_usize 0)
+              l
+              (fun temp_0_ temp_1_ ->
+                  let h0h1, vi:(Alloc.Vec.t_Vec (Alloc.Vec.t_Vec (bool & bool) Alloc.Alloc.t_Global)
+                      Alloc.Alloc.t_Global &
+                    Alloc.Vec.t_Vec bool Alloc.Alloc.t_Global) =
+                    temp_0_
+                  in
+                  let _:usize = temp_1_ in
+                  b2t ((Alloc.Vec.impl_1__len #bool #Alloc.Alloc.t_Global vi <: usize) =. l <: bool) /\
+                  b2t
+                  ((Alloc.Vec.impl_1__len #(Alloc.Vec.t_Vec (bool & bool) Alloc.Alloc.t_Global)
+                        #Alloc.Alloc.t_Global
+                        h0h1
+                      <:
+                      usize) =.
+                    n
+                    <:
+                    bool) /\
+                  (forall (j: usize).
+                      b2t
+                      ((mk_usize 0 <=. j <: bool) && (j <. n <: bool) &&
+                        ((Alloc.Vec.impl_1__len #(Alloc.Vec.t_Vec (bool & bool) Alloc.Alloc.t_Global
+                              )
+                              #Alloc.Alloc.t_Global
+                              h0h1
                             <:
-                            t_Slice u8)
-                      in
-                      let hash_kixj_delta:Blake3.t_Hash =
-                        Blake3.hash (Core.Num.impl_u128__to_le_bytes (kixj.Polytune.Data_types._0 ^.
-                                delta.Polytune.Data_types._0
-                                <:
-                                u128)
+                            usize) =.
+                          n
+                          <:
+                          bool)) ==>
+                      b2t
+                      ((Alloc.Vec.impl_1__len #(bool & bool)
+                            #Alloc.Alloc.t_Global
+                            (h0h1.[ j ] <: Alloc.Vec.t_Vec (bool & bool) Alloc.Alloc.t_Global)
+                          <:
+                          usize) =.
+                        l
+                        <:
+                        bool)))
+              (h0h1, vi
+                <:
+                (Alloc.Vec.t_Vec (Alloc.Vec.t_Vec (bool & bool) Alloc.Alloc.t_Global)
+                    Alloc.Alloc.t_Global &
+                  Alloc.Vec.t_Vec bool Alloc.Alloc.t_Global))
+              (fun temp_0_ ll ->
+                  let h0h1, vi:(Alloc.Vec.t_Vec (Alloc.Vec.t_Vec (bool & bool) Alloc.Alloc.t_Global)
+                      Alloc.Alloc.t_Global &
+                    Alloc.Vec.t_Vec bool Alloc.Alloc.t_Global) =
+                    temp_0_
+                  in
+                  let ll:usize = ll in
+                  let (sj: bool):bool = random_bool () in
+                  let _, kixj:(Polytune.Data_types.t_Mac & Polytune.Data_types.t_Key) =
+                    (xshares.[ ll ] <: Polytune.Data_types.t_Share).Polytune.Data_types._1
+                      .Polytune.Data_types._0.[ j ]
+                  in
+                  let hash_kixj:Blake3.t_Hash =
+                    Blake3.hash (Core.Num.impl_u128__to_le_bytes kixj.Polytune.Data_types._0
+                        <:
+                        t_Slice u8)
+                  in
+                  let hash_kixj_delta:Blake3.t_Hash =
+                    Blake3.hash (Core.Num.impl_u128__to_le_bytes (kixj.Polytune.Data_types._0 ^.
+                            delta.Polytune.Data_types._0
                             <:
-                            t_Slice u8)
-                      in
-                      let h0h1:Alloc.Vec.t_Vec (bool & bool) Alloc.Alloc.t_Global =
-                        Rust_primitives.Hax.Monomorphized_update_at.update_at_usize h0h1
+                            u128)
+                        <:
+                        t_Slice u8)
+                  in
+                  let h0h1:Alloc.Vec.t_Vec (Alloc.Vec.t_Vec (bool & bool) Alloc.Alloc.t_Global)
+                    Alloc.Alloc.t_Global =
+                    Rust_primitives.Hax.Monomorphized_update_at.update_at_usize h0h1
+                      j
+                      (Rust_primitives.Hax.Monomorphized_update_at.update_at_usize (h0h1.[ j ]
+                            <:
+                            Alloc.Vec.t_Vec (bool & bool) Alloc.Alloc.t_Global)
                           ll
                           ({
-                              (h0h1.[ ll ] <: (bool & bool)) with
+                              ((h0h1.[ j ] <: Alloc.Vec.t_Vec (bool & bool) Alloc.Alloc.t_Global).[ ll
+                                ]
+                                <:
+                                (bool & bool)) with
                               _1
                               =
                               Core.Ops.Bit.f_bitxor ((((Blake3.impl_Hash__as_bytes hash_kixj
@@ -306,12 +243,22 @@ let fhaand
                             }
                             <:
                             (bool & bool))
-                      in
-                      let h0h1:Alloc.Vec.t_Vec (bool & bool) Alloc.Alloc.t_Global =
-                        Rust_primitives.Hax.Monomorphized_update_at.update_at_usize h0h1
+                        <:
+                        Alloc.Vec.t_Vec (bool & bool) Alloc.Alloc.t_Global)
+                  in
+                  let h0h1:Alloc.Vec.t_Vec (Alloc.Vec.t_Vec (bool & bool) Alloc.Alloc.t_Global)
+                    Alloc.Alloc.t_Global =
+                    Rust_primitives.Hax.Monomorphized_update_at.update_at_usize h0h1
+                      j
+                      (Rust_primitives.Hax.Monomorphized_update_at.update_at_usize (h0h1.[ j ]
+                            <:
+                            Alloc.Vec.t_Vec (bool & bool) Alloc.Alloc.t_Global)
                           ll
                           ({
-                              (h0h1.[ ll ] <: (bool & bool)) with
+                              ((h0h1.[ j ] <: Alloc.Vec.t_Vec (bool & bool) Alloc.Alloc.t_Global).[ ll
+                                ]
+                                <:
+                                (bool & bool)) with
                               _2
                               =
                               Core.Ops.Bit.f_bitxor (Core.Ops.Bit.f_bitxor ((((Blake3.impl_Hash__as_bytes
@@ -335,231 +282,147 @@ let fhaand
                             }
                             <:
                             (bool & bool))
-                      in
-                      let vi:Alloc.Vec.t_Vec bool Alloc.Alloc.t_Global =
-                        Rust_primitives.Hax.Monomorphized_update_at.update_at_usize vi
-                          ll
-                          (Core.Ops.Bit.f_bitxor (vi.[ ll ] <: bool) sj <: bool)
-                      in
-                      h0h1, vi
-                      <:
-                      (Alloc.Vec.t_Vec (bool & bool) Alloc.Alloc.t_Global &
-                        Alloc.Vec.t_Vec bool Alloc.Alloc.t_Global))
-              in
-              let tmp0, out:(iimpl_951670863_ &
-                Core.Result.t_Result Prims.unit Polytune.Channel.t_Error) =
-                Polytune.Channel.send_to #(bool & bool)
-                  #iimpl_951670863_
-                  channel
-                  j
-                  "haand"
-                  (Core.Ops.Deref.f_deref #(Alloc.Vec.t_Vec (bool & bool) Alloc.Alloc.t_Global)
-                      #FStar.Tactics.Typeclasses.solve
-                      h0h1
-                    <:
-                    t_Slice (bool & bool))
-              in
-              let channel:iimpl_951670863_ = tmp0 in
-              match out <: Core.Result.t_Result Prims.unit Polytune.Channel.t_Error with
-              | Core.Result.Result_Ok _ ->
-                Core.Ops.Control_flow.ControlFlow_Continue
-                (channel, h0h1, vi
-                  <:
-                  (iimpl_951670863_ & Alloc.Vec.t_Vec (bool & bool) Alloc.Alloc.t_Global &
-                    Alloc.Vec.t_Vec bool Alloc.Alloc.t_Global))
-                <:
-                Core.Ops.Control_flow.t_ControlFlow
-                  (Core.Ops.Control_flow.t_ControlFlow
-                      (iimpl_951670863_ &
-                        Core.Result.t_Result (Alloc.Vec.t_Vec bool Alloc.Alloc.t_Global) t_Error)
-                      (Prims.unit &
-                        (iimpl_951670863_ & Alloc.Vec.t_Vec (bool & bool) Alloc.Alloc.t_Global &
-                          Alloc.Vec.t_Vec bool Alloc.Alloc.t_Global)))
-                  (iimpl_951670863_ & Alloc.Vec.t_Vec (bool & bool) Alloc.Alloc.t_Global &
-                    Alloc.Vec.t_Vec bool Alloc.Alloc.t_Global)
-              | Core.Result.Result_Err err ->
-                Core.Ops.Control_flow.ControlFlow_Break
-                (Core.Ops.Control_flow.ControlFlow_Break
-                  (channel,
-                    (Core.Result.Result_Err
-                      (Core.Convert.f_from #t_Error
-                          #Polytune.Channel.t_Error
-                          #FStar.Tactics.Typeclasses.solve
-                          err)
-                      <:
-                      Core.Result.t_Result (Alloc.Vec.t_Vec bool Alloc.Alloc.t_Global) t_Error)
-                    <:
-                    (iimpl_951670863_ &
-                      Core.Result.t_Result (Alloc.Vec.t_Vec bool Alloc.Alloc.t_Global) t_Error))
-                  <:
-                  Core.Ops.Control_flow.t_ControlFlow
-                    (iimpl_951670863_ &
-                      Core.Result.t_Result (Alloc.Vec.t_Vec bool Alloc.Alloc.t_Global) t_Error)
-                    (Prims.unit &
-                      (iimpl_951670863_ & Alloc.Vec.t_Vec (bool & bool) Alloc.Alloc.t_Global &
-                        Alloc.Vec.t_Vec bool Alloc.Alloc.t_Global)))
-                <:
-                Core.Ops.Control_flow.t_ControlFlow
-                  (Core.Ops.Control_flow.t_ControlFlow
-                      (iimpl_951670863_ &
-                        Core.Result.t_Result (Alloc.Vec.t_Vec bool Alloc.Alloc.t_Global) t_Error)
-                      (Prims.unit &
-                        (iimpl_951670863_ & Alloc.Vec.t_Vec (bool & bool) Alloc.Alloc.t_Global &
-                          Alloc.Vec.t_Vec bool Alloc.Alloc.t_Global)))
-                  (iimpl_951670863_ & Alloc.Vec.t_Vec (bool & bool) Alloc.Alloc.t_Global &
-                    Alloc.Vec.t_Vec bool Alloc.Alloc.t_Global))
-      <:
-      Core.Ops.Control_flow.t_ControlFlow
-        (iimpl_951670863_ & Core.Result.t_Result (Alloc.Vec.t_Vec bool Alloc.Alloc.t_Global) t_Error
-        )
-        (iimpl_951670863_ & Alloc.Vec.t_Vec (bool & bool) Alloc.Alloc.t_Global &
-          Alloc.Vec.t_Vec bool Alloc.Alloc.t_Global)
-    with
-    | Core.Ops.Control_flow.ControlFlow_Break ret -> ret
-    | Core.Ops.Control_flow.ControlFlow_Continue (channel, h0h1, vi) ->
-      match
-        Rust_primitives.Hax.Folds.fold_range_return (mk_usize 0)
-          n
-          (fun temp_0_ temp_1_ ->
-              let channel, vi:(iimpl_951670863_ & Alloc.Vec.t_Vec bool Alloc.Alloc.t_Global) =
-                temp_0_
-              in
-              let _:usize = temp_1_ in
-              true)
-          (channel, vi <: (iimpl_951670863_ & Alloc.Vec.t_Vec bool Alloc.Alloc.t_Global))
-          (fun temp_0_ j ->
-              let channel, vi:(iimpl_951670863_ & Alloc.Vec.t_Vec bool Alloc.Alloc.t_Global) =
-                temp_0_
-              in
-              let j:usize = j in
-              if j =. i <: bool
-              then
-                Core.Ops.Control_flow.ControlFlow_Continue
-                (channel, vi <: (iimpl_951670863_ & Alloc.Vec.t_Vec bool Alloc.Alloc.t_Global))
-                <:
-                Core.Ops.Control_flow.t_ControlFlow
-                  (Core.Ops.Control_flow.t_ControlFlow
-                      (iimpl_951670863_ &
-                        Core.Result.t_Result (Alloc.Vec.t_Vec bool Alloc.Alloc.t_Global) t_Error)
-                      (Prims.unit & (iimpl_951670863_ & Alloc.Vec.t_Vec bool Alloc.Alloc.t_Global)))
-                  (iimpl_951670863_ & Alloc.Vec.t_Vec bool Alloc.Alloc.t_Global)
-              else
-                let tmp0, out:(iimpl_951670863_ &
-                  Core.Result.t_Result (Alloc.Vec.t_Vec (bool & bool) Alloc.Alloc.t_Global)
-                    Polytune.Channel.t_Error) =
-                  Polytune.Channel.recv_vec_from #(bool & bool)
-                    #iimpl_951670863_
-                    channel
-                    j
-                    "haand"
-                    l
-                in
-                let channel:iimpl_951670863_ = tmp0 in
-                match
-                  out
-                  <:
-                  Core.Result.t_Result (Alloc.Vec.t_Vec (bool & bool) Alloc.Alloc.t_Global)
-                    Polytune.Channel.t_Error
-                with
-                | Core.Result.Result_Ok h0h1_j ->
-                  let vi:Alloc.Vec.t_Vec bool Alloc.Alloc.t_Global =
-                    Rust_primitives.Hax.Folds.fold_range (mk_usize 0)
-                      l
-                      (fun vi temp_1_ ->
-                          let vi:Alloc.Vec.t_Vec bool Alloc.Alloc.t_Global = vi in
-                          let _:usize = temp_1_ in
-                          true)
-                      vi
-                      (fun vi ll ->
-                          let vi:Alloc.Vec.t_Vec bool Alloc.Alloc.t_Global = vi in
-                          let ll:usize = ll in
-                          let mixj, _:(Polytune.Data_types.t_Mac & Polytune.Data_types.t_Key) =
-                            (xshares.[ ll ] <: Polytune.Data_types.t_Share).Polytune.Data_types._1
-                              .Polytune.Data_types._0.[ j ]
-                          in
-                          let hash_mixj:Blake3.t_Hash =
-                            Blake3.hash (Core.Num.impl_u128__to_le_bytes mixj.Polytune.Data_types._0
-                                <:
-                                t_Slice u8)
-                          in
-                          let t:bool =
-                            (((Blake3.impl_Hash__as_bytes hash_mixj <: t_Array u8 (mk_usize 32)).[ mk_usize
-                                  31 ]
-                                <:
-                                u8) &.
-                              mk_u8 1
-                              <:
-                              u8) <>.
-                            mk_u8 0
-                          in
-                          let t:bool =
-                            Core.Ops.Bit.f_bitxor t
-                              (if
-                                  (xshares.[ ll ] <: Polytune.Data_types.t_Share)
-                                    .Polytune.Data_types._0
-                                then (h0h1_j.[ ll ] <: (bool & bool))._2
-                                else (h0h1_j.[ ll ] <: (bool & bool))._1)
-                          in
-                          let vi:Alloc.Vec.t_Vec bool Alloc.Alloc.t_Global =
-                            Rust_primitives.Hax.Monomorphized_update_at.update_at_usize vi
-                              ll
-                              (Core.Ops.Bit.f_bitxor (vi.[ ll ] <: bool) t <: bool)
-                          in
-                          vi)
-                  in
-                  Core.Ops.Control_flow.ControlFlow_Continue
-                  (channel, vi <: (iimpl_951670863_ & Alloc.Vec.t_Vec bool Alloc.Alloc.t_Global))
-                  <:
-                  Core.Ops.Control_flow.t_ControlFlow
-                    (Core.Ops.Control_flow.t_ControlFlow
-                        (iimpl_951670863_ &
-                          Core.Result.t_Result (Alloc.Vec.t_Vec bool Alloc.Alloc.t_Global) t_Error)
-                        (Prims.unit & (iimpl_951670863_ & Alloc.Vec.t_Vec bool Alloc.Alloc.t_Global)
-                        )) (iimpl_951670863_ & Alloc.Vec.t_Vec bool Alloc.Alloc.t_Global)
-                | Core.Result.Result_Err err ->
-                  Core.Ops.Control_flow.ControlFlow_Break
-                  (Core.Ops.Control_flow.ControlFlow_Break
-                    (channel,
-                      (Core.Result.Result_Err
-                        (Core.Convert.f_from #t_Error
-                            #Polytune.Channel.t_Error
-                            #FStar.Tactics.Typeclasses.solve
-                            err)
                         <:
-                        Core.Result.t_Result (Alloc.Vec.t_Vec bool Alloc.Alloc.t_Global) t_Error)
-                      <:
-                      (iimpl_951670863_ &
-                        Core.Result.t_Result (Alloc.Vec.t_Vec bool Alloc.Alloc.t_Global) t_Error))
-                    <:
-                    Core.Ops.Control_flow.t_ControlFlow
-                      (iimpl_951670863_ &
-                        Core.Result.t_Result (Alloc.Vec.t_Vec bool Alloc.Alloc.t_Global) t_Error)
-                      (Prims.unit & (iimpl_951670863_ & Alloc.Vec.t_Vec bool Alloc.Alloc.t_Global)))
+                        Alloc.Vec.t_Vec (bool & bool) Alloc.Alloc.t_Global)
+                  in
+                  let vi:Alloc.Vec.t_Vec bool Alloc.Alloc.t_Global =
+                    Rust_primitives.Hax.Monomorphized_update_at.update_at_usize vi
+                      ll
+                      (Core.Ops.Bit.f_bitxor (vi.[ ll ] <: bool) sj <: bool)
+                  in
+                  h0h1, vi
                   <:
-                  Core.Ops.Control_flow.t_ControlFlow
-                    (Core.Ops.Control_flow.t_ControlFlow
-                        (iimpl_951670863_ &
-                          Core.Result.t_Result (Alloc.Vec.t_Vec bool Alloc.Alloc.t_Global) t_Error)
-                        (Prims.unit & (iimpl_951670863_ & Alloc.Vec.t_Vec bool Alloc.Alloc.t_Global)
-                        )) (iimpl_951670863_ & Alloc.Vec.t_Vec bool Alloc.Alloc.t_Global))
-        <:
-        Core.Ops.Control_flow.t_ControlFlow
-          (iimpl_951670863_ &
-            Core.Result.t_Result (Alloc.Vec.t_Vec bool Alloc.Alloc.t_Global) t_Error)
-          (iimpl_951670863_ & Alloc.Vec.t_Vec bool Alloc.Alloc.t_Global)
-      with
-      | Core.Ops.Control_flow.ControlFlow_Break ret -> ret
-      | Core.Ops.Control_flow.ControlFlow_Continue (channel, vi) ->
-        let hax_temp_output:Core.Result.t_Result (Alloc.Vec.t_Vec bool Alloc.Alloc.t_Global) t_Error
-        =
-          Core.Result.Result_Ok vi
+                  (Alloc.Vec.t_Vec (Alloc.Vec.t_Vec (bool & bool) Alloc.Alloc.t_Global)
+                      Alloc.Alloc.t_Global &
+                    Alloc.Vec.t_Vec bool Alloc.Alloc.t_Global))
+            <:
+            (Alloc.Vec.t_Vec (Alloc.Vec.t_Vec (bool & bool) Alloc.Alloc.t_Global)
+                Alloc.Alloc.t_Global &
+              Alloc.Vec.t_Vec bool Alloc.Alloc.t_Global))
+  in
+  vi, h0h1
+  <:
+  (Alloc.Vec.t_Vec bool Alloc.Alloc.t_Global &
+    Alloc.Vec.t_Vec (Alloc.Vec.t_Vec (bool & bool) Alloc.Alloc.t_Global) Alloc.Alloc.t_Global)
+
+let fhaand_2_
+      (i n l: usize)
+      (xshares: t_Slice Polytune.Data_types.t_Share)
+      (vi: Alloc.Vec.t_Vec bool Alloc.Alloc.t_Global)
+      (h0h1_j:
+          Alloc.Vec.t_Vec (Alloc.Vec.t_Vec (bool & bool) Alloc.Alloc.t_Global) Alloc.Alloc.t_Global)
+    : Prims.Pure (Alloc.Vec.t_Vec bool Alloc.Alloc.t_Global)
+      (requires
+        b2t ((Alloc.Vec.impl_1__len #bool #Alloc.Alloc.t_Global vi <: usize) =. l <: bool) /\
+        b2t ((Core.Slice.impl__len #Polytune.Data_types.t_Share xshares <: usize) >=. l <: bool) /\
+        (forall (ll: usize).
+            b2t
+            ((mk_usize 0 <=. ll <: bool) && (ll <. l <: bool) &&
+              ((Core.Slice.impl__len #Polytune.Data_types.t_Share xshares <: usize) >=. l <: bool)) ==>
+            b2t
+            ((Alloc.Vec.impl_1__len #(Polytune.Data_types.t_Mac & Polytune.Data_types.t_Key)
+                  #Alloc.Alloc.t_Global
+                  (xshares.[ ll ] <: Polytune.Data_types.t_Share).Polytune.Data_types._1
+                    .Polytune.Data_types._0
+                <:
+                usize) >=.
+              n
+              <:
+              bool)) /\
+        (b2t
+        ((Alloc.Vec.impl_1__len #(Alloc.Vec.t_Vec (bool & bool) Alloc.Alloc.t_Global)
+              #Alloc.Alloc.t_Global
+              h0h1_j
+            <:
+            usize) >=.
+          n
           <:
-          Core.Result.t_Result (Alloc.Vec.t_Vec bool Alloc.Alloc.t_Global) t_Error
-        in
-        channel, hax_temp_output
-        <:
-        (iimpl_951670863_ & Core.Result.t_Result (Alloc.Vec.t_Vec bool Alloc.Alloc.t_Global) t_Error
-        )
+          bool) /\
+        (forall (j: usize).
+            b2t
+            ((mk_usize 0 <=. j <: bool) && (j <. n <: bool) &&
+              ((Alloc.Vec.impl_1__len #(Alloc.Vec.t_Vec (bool & bool) Alloc.Alloc.t_Global)
+                    #Alloc.Alloc.t_Global
+                    h0h1_j
+                  <:
+                  usize) >=.
+                n
+                <:
+                bool)) ==>
+            b2t
+            ((Alloc.Vec.impl_1__len #(bool & bool)
+                  #Alloc.Alloc.t_Global
+                  (h0h1_j.[ j ] <: Alloc.Vec.t_Vec (bool & bool) Alloc.Alloc.t_Global)
+                <:
+                usize) >=.
+              l
+              <:
+              bool))))
+      (fun _ -> Prims.l_True) =
+  Rust_primitives.Hax.Folds.fold_range (mk_usize 0)
+    n
+    (fun vi temp_1_ ->
+        let vi:Alloc.Vec.t_Vec bool Alloc.Alloc.t_Global = vi in
+        let _:usize = temp_1_ in
+        (Alloc.Vec.impl_1__len #bool #Alloc.Alloc.t_Global vi <: usize) =. l <: bool)
+    vi
+    (fun vi j ->
+        let vi:Alloc.Vec.t_Vec bool Alloc.Alloc.t_Global = vi in
+        let j:usize = j in
+        if j =. i <: bool
+        then vi
+        else
+          Rust_primitives.Hax.Folds.fold_range (mk_usize 0)
+            l
+            (fun vi temp_1_ ->
+                let vi:Alloc.Vec.t_Vec bool Alloc.Alloc.t_Global = vi in
+                let _:usize = temp_1_ in
+                (Alloc.Vec.impl_1__len #bool #Alloc.Alloc.t_Global vi <: usize) =. l <: bool)
+            vi
+            (fun vi ll ->
+                let vi:Alloc.Vec.t_Vec bool Alloc.Alloc.t_Global = vi in
+                let ll:usize = ll in
+                let mixj, _:(Polytune.Data_types.t_Mac & Polytune.Data_types.t_Key) =
+                  (xshares.[ ll ] <: Polytune.Data_types.t_Share).Polytune.Data_types._1
+                    .Polytune.Data_types._0.[ j ]
+                in
+                let hash_mixj:Blake3.t_Hash =
+                  Blake3.hash (Core.Num.impl_u128__to_le_bytes mixj.Polytune.Data_types._0
+                      <:
+                      t_Slice u8)
+                in
+                let t:bool =
+                  (((Blake3.impl_Hash__as_bytes hash_mixj <: t_Array u8 (mk_usize 32)).[ mk_usize 31
+                      ]
+                      <:
+                      u8) &.
+                    mk_u8 1
+                    <:
+                    u8) <>.
+                  mk_u8 0
+                in
+                let t:bool =
+                  Core.Ops.Bit.f_bitxor t
+                    (if (xshares.[ ll ] <: Polytune.Data_types.t_Share).Polytune.Data_types._0
+                      then
+                        ((h0h1_j.[ j ] <: Alloc.Vec.t_Vec (bool & bool) Alloc.Alloc.t_Global).[ ll ]
+                          <:
+                          (bool & bool))
+                          ._2
+                      else
+                        ((h0h1_j.[ j ] <: Alloc.Vec.t_Vec (bool & bool) Alloc.Alloc.t_Global).[ ll ]
+                          <:
+                          (bool & bool))
+                          ._1)
+                in
+                let vi:Alloc.Vec.t_Vec bool Alloc.Alloc.t_Global =
+                  Rust_primitives.Hax.Monomorphized_update_at.update_at_usize vi
+                    ll
+                    (Core.Ops.Bit.f_bitxor (vi.[ ll ] <: bool) t <: bool)
+                in
+                vi)
+          <:
+          Alloc.Vec.t_Vec bool Alloc.Alloc.t_Global)
 
 /// This function takes a 128-bit unsigned integer (`u128`) as input and produces a 128-bit hash value.
 /// We use the BLAKE3 cryptographic hash function to hash the input value and return the resulting hash.
@@ -568,1407 +431,1127 @@ let fhaand
 /// resistance. This is sufficient for the purposes of the protocol if RHO <= 64, which we expect
 /// to be the case in all real-world usages of our protocol.
 assume
-val hash128': input: u128 -> Core.Result.t_Result u128 t_Error
+val hash128': input: u128 -> u128
 
 unfold
 let hash128 = hash128'
 
-/// Protocol Pi_LaAND that performs F_LaAND from the paper
-/// [Global-Scale Secure Multiparty Computation](https://dl.acm.org/doi/pdf/10.1145/3133956.3133979).
-/// This asynchronous function implements the \"leaky authenticated AND\" protocol. It computes
-/// shares <x>, <y>, and <z> such that the AND of the XORs of the input values x and y equals
-/// the XOR of the output values z.
-let flaand
-      (#iimpl_951670863_: Type0)
-      (#[FStar.Tactics.Typeclasses.tcresolve ()] i1: Polytune.Channel.t_Channel iimpl_951670863_)
-      (channel: iimpl_951670863_)
+let flaand_1_
       (delta: Polytune.Data_types.t_Delta)
-      (xshares, yshares, rshares:
-          (t_Slice Polytune.Data_types.t_Share & t_Slice Polytune.Data_types.t_Share &
-            t_Slice Polytune.Data_types.t_Share))
-      (i: usize)
-      (n: usize)
-      (l: usize)
-    : (iimpl_951670863_ &
-      Core.Result.t_Result (Alloc.Vec.t_Vec Polytune.Data_types.t_Share Alloc.Alloc.t_Global)
-        t_Error) =
-  if
-    (Core.Slice.impl__len #Polytune.Data_types.t_Share xshares <: usize) <>. l ||
-    (Core.Slice.impl__len #Polytune.Data_types.t_Share yshares <: usize) <>. l ||
-    (Core.Slice.impl__len #Polytune.Data_types.t_Share rshares <: usize) <>. l
-  then
-    channel,
-    (Core.Result.Result_Err (Error_InvalidLength <: t_Error)
-      <:
-      Core.Result.t_Result (Alloc.Vec.t_Vec Polytune.Data_types.t_Share Alloc.Alloc.t_Global)
-        t_Error)
-    <:
-    (iimpl_951670863_ &
-      Core.Result.t_Result (Alloc.Vec.t_Vec Polytune.Data_types.t_Share Alloc.Alloc.t_Global)
-        t_Error)
-  else
-    let y:Alloc.Vec.t_Vec bool Alloc.Alloc.t_Global =
-      Core.Iter.Traits.Iterator.f_collect #(Core.Iter.Adapters.Map.t_Map
-            (Core.Iter.Adapters.Take.t_Take (Core.Slice.Iter.t_Iter Polytune.Data_types.t_Share))
-            (Polytune.Data_types.t_Share -> bool))
-        #FStar.Tactics.Typeclasses.solve
-        #(Alloc.Vec.t_Vec bool Alloc.Alloc.t_Global)
-        (Core.Iter.Traits.Iterator.f_map #(Core.Iter.Adapters.Take.t_Take
-              (Core.Slice.Iter.t_Iter Polytune.Data_types.t_Share))
-            #FStar.Tactics.Typeclasses.solve
-            #bool
-            (Core.Iter.Traits.Iterator.f_take #(Core.Slice.Iter.t_Iter Polytune.Data_types.t_Share)
-                #FStar.Tactics.Typeclasses.solve
-                (Core.Slice.impl__iter #Polytune.Data_types.t_Share yshares
-                  <:
-                  Core.Slice.Iter.t_Iter Polytune.Data_types.t_Share)
-                l
-              <:
-              Core.Iter.Adapters.Take.t_Take (Core.Slice.Iter.t_Iter Polytune.Data_types.t_Share))
-            (fun share ->
-                let share:Polytune.Data_types.t_Share = share in
-                share.Polytune.Data_types._0)
-          <:
-          Core.Iter.Adapters.Map.t_Map
-            (Core.Iter.Adapters.Take.t_Take (Core.Slice.Iter.t_Iter Polytune.Data_types.t_Share))
-            (Polytune.Data_types.t_Share -> bool))
-    in
-    let tmp0, out:(iimpl_951670863_ &
-      Core.Result.t_Result (Alloc.Vec.t_Vec bool Alloc.Alloc.t_Global) t_Error) =
-      fhaand #iimpl_951670863_ channel delta i n l xshares y
-    in
-    let channel:iimpl_951670863_ = tmp0 in
-    match out <: Core.Result.t_Result (Alloc.Vec.t_Vec bool Alloc.Alloc.t_Global) t_Error with
-    | Core.Result.Result_Ok v ->
-      let z:Alloc.Vec.t_Vec bool Alloc.Alloc.t_Global = Alloc.Vec.from_elem #bool false l in
-      let e:Alloc.Vec.t_Vec bool Alloc.Alloc.t_Global = Alloc.Vec.from_elem #bool false l in
-      let zshares:Alloc.Vec.t_Vec Polytune.Data_types.t_Share Alloc.Alloc.t_Global =
-        Alloc.Vec.from_elem #Polytune.Data_types.t_Share
-          (Polytune.Data_types.Share false
-              (Polytune.Data_types.Auth
-                (Alloc.Vec.from_elem #(Polytune.Data_types.t_Mac & Polytune.Data_types.t_Key)
-                    ((Polytune.Data_types.Mac (mk_u128 0) <: Polytune.Data_types.t_Mac),
-                      (Polytune.Data_types.Key (mk_u128 0) <: Polytune.Data_types.t_Key)
-                      <:
-                      (Polytune.Data_types.t_Mac & Polytune.Data_types.t_Key))
-                    n
-                  <:
-                  Alloc.Vec.t_Vec (Polytune.Data_types.t_Mac & Polytune.Data_types.t_Key)
-                    Alloc.Alloc.t_Global)
+      (xshares yshares rshares: t_Slice Polytune.Data_types.t_Share)
+      (i n l: usize)
+      (v: Alloc.Vec.t_Vec bool Alloc.Alloc.t_Global)
+    : Prims.Pure
+      (Core.Result.t_Result
+          (Alloc.Vec.t_Vec (Alloc.Vec.t_Vec u128 Alloc.Alloc.t_Global) Alloc.Alloc.t_Global &
+            Alloc.Vec.t_Vec (Alloc.Vec.t_Vec (bool & u128) Alloc.Alloc.t_Global)
+              Alloc.Alloc.t_Global &
+            Alloc.Vec.t_Vec u128 Alloc.Alloc.t_Global) t_Error)
+      (requires
+        b2t ((Alloc.Vec.impl_1__len #bool #Alloc.Alloc.t_Global v <: usize) >=. l <: bool) /\
+        b2t ((Core.Slice.impl__len #Polytune.Data_types.t_Share rshares <: usize) >=. l <: bool) /\
+        (b2t ((Core.Slice.impl__len #Polytune.Data_types.t_Share xshares <: usize) >=. l <: bool) /\
+        (forall (ll: usize).
+            b2t
+            ((mk_usize 0 <=. ll <: bool) && (ll <. l <: bool) &&
+              ((Core.Slice.impl__len #Polytune.Data_types.t_Share xshares <: usize) >=. l <: bool)) ==>
+            b2t
+            ((Alloc.Vec.impl_1__len #(Polytune.Data_types.t_Mac & Polytune.Data_types.t_Key)
+                  #Alloc.Alloc.t_Global
+                  (xshares.[ ll ] <: Polytune.Data_types.t_Share).Polytune.Data_types._1
+                    .Polytune.Data_types._0
                 <:
-                Polytune.Data_types.t_Auth)
-            <:
-            Polytune.Data_types.t_Share)
-          l
-      in
-      let e, z, zshares:(Alloc.Vec.t_Vec bool Alloc.Alloc.t_Global &
-        Alloc.Vec.t_Vec bool Alloc.Alloc.t_Global &
-        Alloc.Vec.t_Vec Polytune.Data_types.t_Share Alloc.Alloc.t_Global) =
-        Rust_primitives.Hax.Folds.fold_range (mk_usize 0)
-          l
-          (fun temp_0_ temp_1_ ->
-              let e, z, zshares:(Alloc.Vec.t_Vec bool Alloc.Alloc.t_Global &
-                Alloc.Vec.t_Vec bool Alloc.Alloc.t_Global &
-                Alloc.Vec.t_Vec Polytune.Data_types.t_Share Alloc.Alloc.t_Global) =
-                temp_0_
-              in
-              let _:usize = temp_1_ in
-              true)
-          (e, z, zshares
-            <:
-            (Alloc.Vec.t_Vec bool Alloc.Alloc.t_Global & Alloc.Vec.t_Vec bool Alloc.Alloc.t_Global &
-              Alloc.Vec.t_Vec Polytune.Data_types.t_Share Alloc.Alloc.t_Global))
-          (fun temp_0_ ll ->
-              let e, z, zshares:(Alloc.Vec.t_Vec bool Alloc.Alloc.t_Global &
-                Alloc.Vec.t_Vec bool Alloc.Alloc.t_Global &
-                Alloc.Vec.t_Vec Polytune.Data_types.t_Share Alloc.Alloc.t_Global) =
-                temp_0_
-              in
-              let ll:usize = ll in
-              let z:Alloc.Vec.t_Vec bool Alloc.Alloc.t_Global =
-                Rust_primitives.Hax.Monomorphized_update_at.update_at_usize z
-                  ll
-                  (Core.Ops.Bit.f_bitxor (v.[ ll ] <: bool)
-                      (Core.Ops.Bit.f_bitand (xshares.[ ll ] <: Polytune.Data_types.t_Share)
-                            .Polytune.Data_types._0
-                          (yshares.[ ll ] <: Polytune.Data_types.t_Share).Polytune.Data_types._0
+                usize) >=.
+              n
+              <:
+              bool)) /\
+        (b2t ((Core.Slice.impl__len #Polytune.Data_types.t_Share yshares <: usize) >=. l <: bool) /\
+        (forall (ll: usize).
+            b2t
+            ((mk_usize 0 <=. ll <: bool) && (ll <. l <: bool) &&
+              ((Core.Slice.impl__len #Polytune.Data_types.t_Share yshares <: usize) >=. l <: bool)) ==>
+            b2t
+            ((Alloc.Vec.impl_1__len #(Polytune.Data_types.t_Mac & Polytune.Data_types.t_Key)
+                  #Alloc.Alloc.t_Global
+                  (yshares.[ ll ] <: Polytune.Data_types.t_Share).Polytune.Data_types._1
+                    .Polytune.Data_types._0
+                <:
+                usize) >=.
+              n
+              <:
+              bool)))))
+      (fun _ -> Prims.l_True) =
+  let z:Alloc.Vec.t_Vec bool Alloc.Alloc.t_Global = Alloc.Vec.from_elem #bool false l in
+  let e:Alloc.Vec.t_Vec bool Alloc.Alloc.t_Global = Alloc.Vec.from_elem #bool false l in
+  let e, z:(Alloc.Vec.t_Vec bool Alloc.Alloc.t_Global & Alloc.Vec.t_Vec bool Alloc.Alloc.t_Global) =
+    Rust_primitives.Hax.Folds.fold_range (mk_usize 0)
+      l
+      (fun temp_0_ temp_1_ ->
+          let e, z:(Alloc.Vec.t_Vec bool Alloc.Alloc.t_Global &
+            Alloc.Vec.t_Vec bool Alloc.Alloc.t_Global) =
+            temp_0_
+          in
+          let _:usize = temp_1_ in
+          ((Alloc.Vec.impl_1__len #bool #Alloc.Alloc.t_Global z <: usize) =. l <: bool) &&
+          ((Alloc.Vec.impl_1__len #bool #Alloc.Alloc.t_Global e <: usize) =. l <: bool))
+      (e, z
+        <:
+        (Alloc.Vec.t_Vec bool Alloc.Alloc.t_Global & Alloc.Vec.t_Vec bool Alloc.Alloc.t_Global))
+      (fun temp_0_ ll ->
+          let e, z:(Alloc.Vec.t_Vec bool Alloc.Alloc.t_Global &
+            Alloc.Vec.t_Vec bool Alloc.Alloc.t_Global) =
+            temp_0_
+          in
+          let ll:usize = ll in
+          let z:Alloc.Vec.t_Vec bool Alloc.Alloc.t_Global =
+            Rust_primitives.Hax.Monomorphized_update_at.update_at_usize z
+              ll
+              (Core.Ops.Bit.f_bitxor (v.[ ll ] <: bool)
+                  (Core.Ops.Bit.f_bitand (xshares.[ ll ] <: Polytune.Data_types.t_Share)
+                        .Polytune.Data_types._0
+                      (yshares.[ ll ] <: Polytune.Data_types.t_Share).Polytune.Data_types._0
+                    <:
+                    bool)
+                <:
+                bool)
+          in
+          let e:Alloc.Vec.t_Vec bool Alloc.Alloc.t_Global =
+            Rust_primitives.Hax.Monomorphized_update_at.update_at_usize e
+              ll
+              (Core.Ops.Bit.f_bitxor (z.[ ll ] <: bool)
+                  (rshares.[ ll ] <: Polytune.Data_types.t_Share).Polytune.Data_types._0
+                <:
+                bool)
+          in
+          e, z
+          <:
+          (Alloc.Vec.t_Vec bool Alloc.Alloc.t_Global & Alloc.Vec.t_Vec bool Alloc.Alloc.t_Global))
+  in
+  let phi:Alloc.Vec.t_Vec u128 Alloc.Alloc.t_Global = Alloc.Vec.from_elem #u128 (mk_u128 0) l in
+  let phi:Alloc.Vec.t_Vec u128 Alloc.Alloc.t_Global =
+    Rust_primitives.Hax.Folds.fold_range (mk_usize 0)
+      l
+      (fun phi temp_1_ ->
+          let phi:Alloc.Vec.t_Vec u128 Alloc.Alloc.t_Global = phi in
+          let _:usize = temp_1_ in
+          (Alloc.Vec.impl_1__len #u128 #Alloc.Alloc.t_Global phi <: usize) =. l <: bool)
+      phi
+      (fun phi ll ->
+          let phi:Alloc.Vec.t_Vec u128 Alloc.Alloc.t_Global = phi in
+          let ll:usize = ll in
+          let phi:Alloc.Vec.t_Vec u128 Alloc.Alloc.t_Global =
+            Rust_primitives.Hax.Folds.fold_range (mk_usize 0)
+              n
+              (fun phi temp_1_ ->
+                  let phi:Alloc.Vec.t_Vec u128 Alloc.Alloc.t_Global = phi in
+                  let _:usize = temp_1_ in
+                  (Alloc.Vec.impl_1__len #u128 #Alloc.Alloc.t_Global phi <: usize) =. l <: bool)
+              phi
+              (fun phi k ->
+                  let phi:Alloc.Vec.t_Vec u128 Alloc.Alloc.t_Global = phi in
+                  let k:usize = k in
+                  if k =. i <: bool
+                  then phi
+                  else
+                    let mk_yi, ki_yk:(Polytune.Data_types.t_Mac & Polytune.Data_types.t_Key) =
+                      (yshares.[ ll ] <: Polytune.Data_types.t_Share).Polytune.Data_types._1
+                        .Polytune.Data_types._0.[ k ]
+                    in
+                    let phi:Alloc.Vec.t_Vec u128 Alloc.Alloc.t_Global =
+                      Rust_primitives.Hax.Monomorphized_update_at.update_at_usize phi
+                        ll
+                        (((phi.[ ll ] <: u128) ^. ki_yk.Polytune.Data_types._0 <: u128) ^.
+                          mk_yi.Polytune.Data_types._0
+                          <:
+                          u128)
+                    in
+                    phi)
+          in
+          let phi:Alloc.Vec.t_Vec u128 Alloc.Alloc.t_Global =
+            Rust_primitives.Hax.Monomorphized_update_at.update_at_usize phi
+              ll
+              ((phi.[ ll ] <: u128) ^.
+                ((cast ((yshares.[ ll ] <: Polytune.Data_types.t_Share).Polytune.Data_types._0
                         <:
                         bool)
                     <:
-                    bool)
-              in
-              let e:Alloc.Vec.t_Vec bool Alloc.Alloc.t_Global =
-                Rust_primitives.Hax.Monomorphized_update_at.update_at_usize e
-                  ll
-                  (Core.Ops.Bit.f_bitxor (z.[ ll ] <: bool)
-                      (rshares.[ ll ] <: Polytune.Data_types.t_Share).Polytune.Data_types._0
-                    <:
-                    bool)
-              in
-              let zshares:Alloc.Vec.t_Vec Polytune.Data_types.t_Share Alloc.Alloc.t_Global =
-                Rust_primitives.Hax.Monomorphized_update_at.update_at_usize zshares
-                  ll
-                  ({
-                      (zshares.[ ll ] <: Polytune.Data_types.t_Share) with
-                      Polytune.Data_types._0 = z.[ ll ] <: bool
-                    }
-                    <:
-                    Polytune.Data_types.t_Share)
-              in
-              e, z, zshares
-              <:
-              (Alloc.Vec.t_Vec bool Alloc.Alloc.t_Global & Alloc.Vec.t_Vec bool Alloc.Alloc.t_Global &
-                Alloc.Vec.t_Vec Polytune.Data_types.t_Share Alloc.Alloc.t_Global))
-      in
-      let phi:Alloc.Vec.t_Vec u128 Alloc.Alloc.t_Global = Alloc.Vec.from_elem #u128 (mk_u128 0) l in
-      let phi:Alloc.Vec.t_Vec u128 Alloc.Alloc.t_Global =
-        Rust_primitives.Hax.Folds.fold_range (mk_usize 0)
-          l
-          (fun phi temp_1_ ->
-              let phi:Alloc.Vec.t_Vec u128 Alloc.Alloc.t_Global = phi in
-              let _:usize = temp_1_ in
-              true)
-          phi
-          (fun phi ll ->
-              let phi:Alloc.Vec.t_Vec u128 Alloc.Alloc.t_Global = phi in
-              let ll:usize = ll in
-              let phi:Alloc.Vec.t_Vec u128 Alloc.Alloc.t_Global =
-                Rust_primitives.Hax.Folds.fold_range (mk_usize 0)
-                  n
-                  (fun phi temp_1_ ->
-                      let phi:Alloc.Vec.t_Vec u128 Alloc.Alloc.t_Global = phi in
-                      let _:usize = temp_1_ in
-                      true)
-                  phi
-                  (fun phi k ->
-                      let phi:Alloc.Vec.t_Vec u128 Alloc.Alloc.t_Global = phi in
-                      let k:usize = k in
-                      if k =. i <: bool
-                      then phi
-                      else
-                        let mk_yi, ki_yk:(Polytune.Data_types.t_Mac & Polytune.Data_types.t_Key) =
-                          (yshares.[ ll ] <: Polytune.Data_types.t_Share).Polytune.Data_types._1
-                            .Polytune.Data_types._0.[ k ]
-                        in
-                        let phi:Alloc.Vec.t_Vec u128 Alloc.Alloc.t_Global =
-                          Rust_primitives.Hax.Monomorphized_update_at.update_at_usize phi
-                            ll
-                            (((phi.[ ll ] <: u128) ^. ki_yk.Polytune.Data_types._0 <: u128) ^.
-                              mk_yi.Polytune.Data_types._0
-                              <:
-                              u128)
-                        in
-                        phi)
-              in
-              let phi:Alloc.Vec.t_Vec u128 Alloc.Alloc.t_Global =
-                Rust_primitives.Hax.Monomorphized_update_at.update_at_usize phi
-                  ll
-                  ((phi.[ ll ] <: u128) ^.
-                    ((cast ((yshares.[ ll ] <: Polytune.Data_types.t_Share).Polytune.Data_types._0
-                            <:
-                            bool)
-                        <:
-                        u128) *!
-                      delta.Polytune.Data_types._0
-                      <:
-                      u128)
-                    <:
-                    u128)
-              in
-              phi)
-      in
-      let ki_xj_phi:Alloc.Vec.t_Vec (Alloc.Vec.t_Vec u128 Alloc.Alloc.t_Global) Alloc.Alloc.t_Global
-      =
-        Alloc.Vec.from_elem #(Alloc.Vec.t_Vec u128 Alloc.Alloc.t_Global)
-          (Alloc.Vec.from_elem #u128 (mk_u128 0) l <: Alloc.Vec.t_Vec u128 Alloc.Alloc.t_Global)
-          n
-      in
-      let ei_uij:Alloc.Vec.t_Vec (Alloc.Vec.t_Vec (bool & u128) Alloc.Alloc.t_Global)
-        Alloc.Alloc.t_Global =
-        Alloc.Vec.from_elem #(Alloc.Vec.t_Vec (bool & u128) Alloc.Alloc.t_Global)
-          (Alloc.Vec.impl__new #(bool & u128) ()
-            <:
-            Alloc.Vec.t_Vec (bool & u128) Alloc.Alloc.t_Global)
-          n
-      in
-      (match
-          Rust_primitives.Hax.Folds.fold_range_return (mk_usize 0)
-            n
-            (fun temp_0_ temp_1_ ->
-                let ei_uij, ki_xj_phi:(Alloc.Vec.t_Vec
-                    (Alloc.Vec.t_Vec (bool & u128) Alloc.Alloc.t_Global) Alloc.Alloc.t_Global &
-                  Alloc.Vec.t_Vec (Alloc.Vec.t_Vec u128 Alloc.Alloc.t_Global) Alloc.Alloc.t_Global)
-                =
-                  temp_0_
-                in
-                let _:usize = temp_1_ in
-                true)
-            (ei_uij, ki_xj_phi
-              <:
-              (Alloc.Vec.t_Vec (Alloc.Vec.t_Vec (bool & u128) Alloc.Alloc.t_Global)
-                  Alloc.Alloc.t_Global &
-                Alloc.Vec.t_Vec (Alloc.Vec.t_Vec u128 Alloc.Alloc.t_Global) Alloc.Alloc.t_Global))
-            (fun temp_0_ j ->
-                let ei_uij, ki_xj_phi:(Alloc.Vec.t_Vec
-                    (Alloc.Vec.t_Vec (bool & u128) Alloc.Alloc.t_Global) Alloc.Alloc.t_Global &
-                  Alloc.Vec.t_Vec (Alloc.Vec.t_Vec u128 Alloc.Alloc.t_Global) Alloc.Alloc.t_Global)
-                =
-                  temp_0_
-                in
-                let j:usize = j in
-                if j =. i <: bool
-                then
-                  Core.Ops.Control_flow.ControlFlow_Continue
-                  (ei_uij, ki_xj_phi
-                    <:
-                    (Alloc.Vec.t_Vec (Alloc.Vec.t_Vec (bool & u128) Alloc.Alloc.t_Global)
-                        Alloc.Alloc.t_Global &
-                      Alloc.Vec.t_Vec (Alloc.Vec.t_Vec u128 Alloc.Alloc.t_Global)
-                        Alloc.Alloc.t_Global))
+                    u128) *!
+                  delta.Polytune.Data_types._0
                   <:
-                  Core.Ops.Control_flow.t_ControlFlow
-                    (Core.Ops.Control_flow.t_ControlFlow
-                        (iimpl_951670863_ &
-                          Core.Result.t_Result
-                            (Alloc.Vec.t_Vec Polytune.Data_types.t_Share Alloc.Alloc.t_Global)
-                            t_Error)
-                        (Prims.unit &
-                          (Alloc.Vec.t_Vec (Alloc.Vec.t_Vec (bool & u128) Alloc.Alloc.t_Global)
-                              Alloc.Alloc.t_Global &
-                            Alloc.Vec.t_Vec (Alloc.Vec.t_Vec u128 Alloc.Alloc.t_Global)
-                              Alloc.Alloc.t_Global)))
-                    (Alloc.Vec.t_Vec (Alloc.Vec.t_Vec (bool & u128) Alloc.Alloc.t_Global)
-                        Alloc.Alloc.t_Global &
-                      Alloc.Vec.t_Vec (Alloc.Vec.t_Vec u128 Alloc.Alloc.t_Global)
-                        Alloc.Alloc.t_Global)
-                else
-                  match
-                    Rust_primitives.Hax.Folds.fold_return (Core.Iter.Traits.Collect.f_into_iter #(Core.Iter.Adapters.Take.t_Take
-                            (Core.Iter.Adapters.Enumerate.t_Enumerate (Core.Slice.Iter.t_Iter u128))
-                          )
-                          #FStar.Tactics.Typeclasses.solve
-                          (Core.Iter.Traits.Iterator.f_take #(Core.Iter.Adapters.Enumerate.t_Enumerate
-                                (Core.Slice.Iter.t_Iter u128))
-                              #FStar.Tactics.Typeclasses.solve
-                              (Core.Iter.Traits.Iterator.f_enumerate #(Core.Slice.Iter.t_Iter u128)
-                                  #FStar.Tactics.Typeclasses.solve
-                                  (Core.Slice.impl__iter #u128
-                                      (Core.Ops.Deref.f_deref #(Alloc.Vec.t_Vec u128
-                                              Alloc.Alloc.t_Global)
-                                          #FStar.Tactics.Typeclasses.solve
-                                          phi
-                                        <:
-                                        t_Slice u128)
-                                    <:
-                                    Core.Slice.Iter.t_Iter u128)
-                                <:
-                                Core.Iter.Adapters.Enumerate.t_Enumerate
-                                (Core.Slice.Iter.t_Iter u128))
-                              l
-                            <:
-                            Core.Iter.Adapters.Take.t_Take
-                            (Core.Iter.Adapters.Enumerate.t_Enumerate (Core.Slice.Iter.t_Iter u128))
-                          )
-                        <:
-                        Core.Iter.Adapters.Take.t_Take
-                        (Core.Iter.Adapters.Enumerate.t_Enumerate (Core.Slice.Iter.t_Iter u128)))
-                      (ei_uij, ki_xj_phi
-                        <:
-                        (Alloc.Vec.t_Vec (Alloc.Vec.t_Vec (bool & u128) Alloc.Alloc.t_Global)
-                            Alloc.Alloc.t_Global &
-                          Alloc.Vec.t_Vec (Alloc.Vec.t_Vec u128 Alloc.Alloc.t_Global)
-                            Alloc.Alloc.t_Global))
-                      (fun temp_0_ temp_1_ ->
-                          let ei_uij, ki_xj_phi:(Alloc.Vec.t_Vec
-                              (Alloc.Vec.t_Vec (bool & u128) Alloc.Alloc.t_Global)
-                              Alloc.Alloc.t_Global &
-                            Alloc.Vec.t_Vec (Alloc.Vec.t_Vec u128 Alloc.Alloc.t_Global)
-                              Alloc.Alloc.t_Global) =
-                            temp_0_
-                          in
-                          let ll, phi_l:(usize & u128) = temp_1_ in
-                          let _, ki_xj:(Polytune.Data_types.t_Mac & Polytune.Data_types.t_Key) =
-                            (xshares.[ ll ] <: Polytune.Data_types.t_Share).Polytune.Data_types._1
-                              .Polytune.Data_types._0.[ j ]
-                          in
-                          match
-                            hash128 ki_xj.Polytune.Data_types._0
-                            <:
-                            Core.Result.t_Result u128 t_Error
-                          with
-                          | Core.Result.Result_Ok hoist9 ->
-                            let ki_xj_phi:Alloc.Vec.t_Vec
-                              (Alloc.Vec.t_Vec u128 Alloc.Alloc.t_Global) Alloc.Alloc.t_Global =
-                              Rust_primitives.Hax.Monomorphized_update_at.update_at_usize ki_xj_phi
-                                j
-                                (Rust_primitives.Hax.Monomorphized_update_at.update_at_usize (ki_xj_phi.[
-                                        j ]
-                                      <:
-                                      Alloc.Vec.t_Vec u128 Alloc.Alloc.t_Global)
-                                    ll
-                                    hoist9
-                                  <:
-                                  Alloc.Vec.t_Vec u128 Alloc.Alloc.t_Global)
-                            in
-                            (match
-                                hash128 (ki_xj.Polytune.Data_types._0 ^.
-                                    delta.Polytune.Data_types._0
-                                    <:
-                                    u128)
-                                <:
-                                Core.Result.t_Result u128 t_Error
-                              with
-                              | Core.Result.Result_Ok hoist12 ->
-                                let uij:u128 =
-                                  (hoist12 ^.
-                                    ((ki_xj_phi.[ j ] <: Alloc.Vec.t_Vec u128 Alloc.Alloc.t_Global).[
-                                        ll ]
-                                      <:
-                                      u128)
-                                    <:
-                                    u128) ^.
-                                  phi_l
-                                in
-                                let ei_uij:Alloc.Vec.t_Vec
-                                  (Alloc.Vec.t_Vec (bool & u128) Alloc.Alloc.t_Global)
-                                  Alloc.Alloc.t_Global =
-                                  Rust_primitives.Hax.Monomorphized_update_at.update_at_usize ei_uij
-                                    j
-                                    (Alloc.Vec.impl_1__push #(bool & u128)
-                                        #Alloc.Alloc.t_Global
-                                        (ei_uij.[ j ]
-                                          <:
-                                          Alloc.Vec.t_Vec (bool & u128) Alloc.Alloc.t_Global)
-                                        ((e.[ ll ] <: bool), uij <: (bool & u128))
-                                      <:
-                                      Alloc.Vec.t_Vec (bool & u128) Alloc.Alloc.t_Global)
-                                in
-                                Core.Ops.Control_flow.ControlFlow_Continue
-                                (ei_uij, ki_xj_phi
-                                  <:
-                                  (Alloc.Vec.t_Vec
-                                      (Alloc.Vec.t_Vec (bool & u128) Alloc.Alloc.t_Global)
-                                      Alloc.Alloc.t_Global &
-                                    Alloc.Vec.t_Vec (Alloc.Vec.t_Vec u128 Alloc.Alloc.t_Global)
-                                      Alloc.Alloc.t_Global))
-                                <:
-                                Core.Ops.Control_flow.t_ControlFlow
-                                  (Core.Ops.Control_flow.t_ControlFlow
-                                      (iimpl_951670863_ &
-                                        Core.Result.t_Result
-                                          (Alloc.Vec.t_Vec Polytune.Data_types.t_Share
-                                              Alloc.Alloc.t_Global) t_Error)
-                                      (Prims.unit &
-                                        (Alloc.Vec.t_Vec
-                                            (Alloc.Vec.t_Vec (bool & u128) Alloc.Alloc.t_Global)
-                                            Alloc.Alloc.t_Global &
-                                          Alloc.Vec.t_Vec
-                                            (Alloc.Vec.t_Vec u128 Alloc.Alloc.t_Global)
-                                            Alloc.Alloc.t_Global)))
-                                  (Alloc.Vec.t_Vec
-                                      (Alloc.Vec.t_Vec (bool & u128) Alloc.Alloc.t_Global)
-                                      Alloc.Alloc.t_Global &
-                                    Alloc.Vec.t_Vec (Alloc.Vec.t_Vec u128 Alloc.Alloc.t_Global)
-                                      Alloc.Alloc.t_Global)
-                              | Core.Result.Result_Err err ->
-                                Core.Ops.Control_flow.ControlFlow_Break
-                                (Core.Ops.Control_flow.ControlFlow_Break
-                                  (channel,
-                                    (Core.Result.Result_Err err
-                                      <:
-                                      Core.Result.t_Result
-                                        (Alloc.Vec.t_Vec Polytune.Data_types.t_Share
-                                            Alloc.Alloc.t_Global) t_Error)
-                                    <:
-                                    (iimpl_951670863_ &
-                                      Core.Result.t_Result
-                                        (Alloc.Vec.t_Vec Polytune.Data_types.t_Share
-                                            Alloc.Alloc.t_Global) t_Error))
-                                  <:
-                                  Core.Ops.Control_flow.t_ControlFlow
-                                    (iimpl_951670863_ &
-                                      Core.Result.t_Result
-                                        (Alloc.Vec.t_Vec Polytune.Data_types.t_Share
-                                            Alloc.Alloc.t_Global) t_Error)
-                                    (Prims.unit &
-                                      (Alloc.Vec.t_Vec
-                                          (Alloc.Vec.t_Vec (bool & u128) Alloc.Alloc.t_Global)
-                                          Alloc.Alloc.t_Global &
-                                        Alloc.Vec.t_Vec (Alloc.Vec.t_Vec u128 Alloc.Alloc.t_Global)
-                                          Alloc.Alloc.t_Global)))
-                                <:
-                                Core.Ops.Control_flow.t_ControlFlow
-                                  (Core.Ops.Control_flow.t_ControlFlow
-                                      (iimpl_951670863_ &
-                                        Core.Result.t_Result
-                                          (Alloc.Vec.t_Vec Polytune.Data_types.t_Share
-                                              Alloc.Alloc.t_Global) t_Error)
-                                      (Prims.unit &
-                                        (Alloc.Vec.t_Vec
-                                            (Alloc.Vec.t_Vec (bool & u128) Alloc.Alloc.t_Global)
-                                            Alloc.Alloc.t_Global &
-                                          Alloc.Vec.t_Vec
-                                            (Alloc.Vec.t_Vec u128 Alloc.Alloc.t_Global)
-                                            Alloc.Alloc.t_Global)))
-                                  (Alloc.Vec.t_Vec
-                                      (Alloc.Vec.t_Vec (bool & u128) Alloc.Alloc.t_Global)
-                                      Alloc.Alloc.t_Global &
-                                    Alloc.Vec.t_Vec (Alloc.Vec.t_Vec u128 Alloc.Alloc.t_Global)
-                                      Alloc.Alloc.t_Global))
-                          | Core.Result.Result_Err err ->
-                            Core.Ops.Control_flow.ControlFlow_Break
-                            (Core.Ops.Control_flow.ControlFlow_Break
-                              (channel,
-                                (Core.Result.Result_Err err
-                                  <:
-                                  Core.Result.t_Result
-                                    (Alloc.Vec.t_Vec Polytune.Data_types.t_Share
-                                        Alloc.Alloc.t_Global) t_Error)
-                                <:
-                                (iimpl_951670863_ &
-                                  Core.Result.t_Result
-                                    (Alloc.Vec.t_Vec Polytune.Data_types.t_Share
-                                        Alloc.Alloc.t_Global) t_Error))
-                              <:
-                              Core.Ops.Control_flow.t_ControlFlow
-                                (iimpl_951670863_ &
-                                  Core.Result.t_Result
-                                    (Alloc.Vec.t_Vec Polytune.Data_types.t_Share
-                                        Alloc.Alloc.t_Global) t_Error)
-                                (Prims.unit &
-                                  (Alloc.Vec.t_Vec
-                                      (Alloc.Vec.t_Vec (bool & u128) Alloc.Alloc.t_Global)
-                                      Alloc.Alloc.t_Global &
-                                    Alloc.Vec.t_Vec (Alloc.Vec.t_Vec u128 Alloc.Alloc.t_Global)
-                                      Alloc.Alloc.t_Global)))
-                            <:
-                            Core.Ops.Control_flow.t_ControlFlow
-                              (Core.Ops.Control_flow.t_ControlFlow
-                                  (iimpl_951670863_ &
-                                    Core.Result.t_Result
-                                      (Alloc.Vec.t_Vec Polytune.Data_types.t_Share
-                                          Alloc.Alloc.t_Global) t_Error)
-                                  (Prims.unit &
-                                    (Alloc.Vec.t_Vec
-                                        (Alloc.Vec.t_Vec (bool & u128) Alloc.Alloc.t_Global)
-                                        Alloc.Alloc.t_Global &
-                                      Alloc.Vec.t_Vec (Alloc.Vec.t_Vec u128 Alloc.Alloc.t_Global)
-                                        Alloc.Alloc.t_Global)))
-                              (Alloc.Vec.t_Vec (Alloc.Vec.t_Vec (bool & u128) Alloc.Alloc.t_Global)
-                                  Alloc.Alloc.t_Global &
-                                Alloc.Vec.t_Vec (Alloc.Vec.t_Vec u128 Alloc.Alloc.t_Global)
-                                  Alloc.Alloc.t_Global))
+                  u128)
+                <:
+                u128)
+          in
+          phi)
+  in
+  let ki_xj_phi:Alloc.Vec.t_Vec (Alloc.Vec.t_Vec u128 Alloc.Alloc.t_Global) Alloc.Alloc.t_Global =
+    Alloc.Vec.from_elem #(Alloc.Vec.t_Vec u128 Alloc.Alloc.t_Global)
+      (Alloc.Vec.from_elem #u128 (mk_u128 0) l <: Alloc.Vec.t_Vec u128 Alloc.Alloc.t_Global)
+      n
+  in
+  let ei_uij:Alloc.Vec.t_Vec (Alloc.Vec.t_Vec (bool & u128) Alloc.Alloc.t_Global)
+    Alloc.Alloc.t_Global =
+    Alloc.Vec.from_elem #(Alloc.Vec.t_Vec (bool & u128) Alloc.Alloc.t_Global)
+      (Alloc.Vec.impl__new #(bool & u128) () <: Alloc.Vec.t_Vec (bool & u128) Alloc.Alloc.t_Global)
+      n
+  in
+  let ei_uij, ki_xj_phi:(Alloc.Vec.t_Vec (Alloc.Vec.t_Vec (bool & u128) Alloc.Alloc.t_Global)
+      Alloc.Alloc.t_Global &
+    Alloc.Vec.t_Vec (Alloc.Vec.t_Vec u128 Alloc.Alloc.t_Global) Alloc.Alloc.t_Global) =
+    Rust_primitives.Hax.Folds.fold_range (mk_usize 0)
+      n
+      (fun temp_0_ temp_1_ ->
+          let ei_uij, ki_xj_phi:(Alloc.Vec.t_Vec
+              (Alloc.Vec.t_Vec (bool & u128) Alloc.Alloc.t_Global) Alloc.Alloc.t_Global &
+            Alloc.Vec.t_Vec (Alloc.Vec.t_Vec u128 Alloc.Alloc.t_Global) Alloc.Alloc.t_Global) =
+            temp_0_
+          in
+          let _:usize = temp_1_ in
+          b2t
+          (((Alloc.Vec.impl_1__len #(Alloc.Vec.t_Vec u128 Alloc.Alloc.t_Global)
+                  #Alloc.Alloc.t_Global
+                  ki_xj_phi
+                <:
+                usize) =.
+              n
+              <:
+              bool) &&
+            ((Alloc.Vec.impl_1__len #(Alloc.Vec.t_Vec (bool & u128) Alloc.Alloc.t_Global)
+                  #Alloc.Alloc.t_Global
+                  ei_uij
+                <:
+                usize) =.
+              n
+              <:
+              bool) &&
+            ((Alloc.Vec.impl_1__len #u128 #Alloc.Alloc.t_Global phi <: usize) =. l <: bool)) /\
+          (forall (j: usize).
+              b2t
+              ((mk_usize 0 <=. j <: bool) && (j <. n <: bool) &&
+                ((Alloc.Vec.impl_1__len #(Alloc.Vec.t_Vec u128 Alloc.Alloc.t_Global)
+                      #Alloc.Alloc.t_Global
+                      ki_xj_phi
                     <:
-                    Core.Ops.Control_flow.t_ControlFlow
-                      (iimpl_951670863_ &
-                        Core.Result.t_Result
-                          (Alloc.Vec.t_Vec Polytune.Data_types.t_Share Alloc.Alloc.t_Global) t_Error
-                      )
-                      (Alloc.Vec.t_Vec (Alloc.Vec.t_Vec (bool & u128) Alloc.Alloc.t_Global)
-                          Alloc.Alloc.t_Global &
-                        Alloc.Vec.t_Vec (Alloc.Vec.t_Vec u128 Alloc.Alloc.t_Global)
-                          Alloc.Alloc.t_Global)
-                  with
-                  | Core.Ops.Control_flow.ControlFlow_Break ret ->
-                    Core.Ops.Control_flow.ControlFlow_Break
-                    (Core.Ops.Control_flow.ControlFlow_Break ret
-                      <:
-                      Core.Ops.Control_flow.t_ControlFlow
-                        (iimpl_951670863_ &
-                          Core.Result.t_Result
-                            (Alloc.Vec.t_Vec Polytune.Data_types.t_Share Alloc.Alloc.t_Global)
-                            t_Error)
-                        (Prims.unit &
-                          (Alloc.Vec.t_Vec (Alloc.Vec.t_Vec (bool & u128) Alloc.Alloc.t_Global)
-                              Alloc.Alloc.t_Global &
-                            Alloc.Vec.t_Vec (Alloc.Vec.t_Vec u128 Alloc.Alloc.t_Global)
-                              Alloc.Alloc.t_Global)))
-                    <:
-                    Core.Ops.Control_flow.t_ControlFlow
-                      (Core.Ops.Control_flow.t_ControlFlow
-                          (iimpl_951670863_ &
-                            Core.Result.t_Result
-                              (Alloc.Vec.t_Vec Polytune.Data_types.t_Share Alloc.Alloc.t_Global)
-                              t_Error)
-                          (Prims.unit &
-                            (Alloc.Vec.t_Vec (Alloc.Vec.t_Vec (bool & u128) Alloc.Alloc.t_Global)
-                                Alloc.Alloc.t_Global &
-                              Alloc.Vec.t_Vec (Alloc.Vec.t_Vec u128 Alloc.Alloc.t_Global)
-                                Alloc.Alloc.t_Global)))
-                      (Alloc.Vec.t_Vec (Alloc.Vec.t_Vec (bool & u128) Alloc.Alloc.t_Global)
-                          Alloc.Alloc.t_Global &
-                        Alloc.Vec.t_Vec (Alloc.Vec.t_Vec u128 Alloc.Alloc.t_Global)
-                          Alloc.Alloc.t_Global)
-                  | Core.Ops.Control_flow.ControlFlow_Continue loop_res ->
-                    Core.Ops.Control_flow.ControlFlow_Continue loop_res
-                    <:
-                    Core.Ops.Control_flow.t_ControlFlow
-                      (Core.Ops.Control_flow.t_ControlFlow
-                          (iimpl_951670863_ &
-                            Core.Result.t_Result
-                              (Alloc.Vec.t_Vec Polytune.Data_types.t_Share Alloc.Alloc.t_Global)
-                              t_Error)
-                          (Prims.unit &
-                            (Alloc.Vec.t_Vec (Alloc.Vec.t_Vec (bool & u128) Alloc.Alloc.t_Global)
-                                Alloc.Alloc.t_Global &
-                              Alloc.Vec.t_Vec (Alloc.Vec.t_Vec u128 Alloc.Alloc.t_Global)
-                                Alloc.Alloc.t_Global)))
-                      (Alloc.Vec.t_Vec (Alloc.Vec.t_Vec (bool & u128) Alloc.Alloc.t_Global)
-                          Alloc.Alloc.t_Global &
-                        Alloc.Vec.t_Vec (Alloc.Vec.t_Vec u128 Alloc.Alloc.t_Global)
-                          Alloc.Alloc.t_Global))
-          <:
-          Core.Ops.Control_flow.t_ControlFlow
-            (iimpl_951670863_ &
-              Core.Result.t_Result
-                (Alloc.Vec.t_Vec Polytune.Data_types.t_Share Alloc.Alloc.t_Global) t_Error)
+                    usize) =.
+                  n
+                  <:
+                  bool)) ==>
+              b2t
+              ((Alloc.Vec.impl_1__len #u128
+                    #Alloc.Alloc.t_Global
+                    (ki_xj_phi.[ j ] <: Alloc.Vec.t_Vec u128 Alloc.Alloc.t_Global)
+                  <:
+                  usize) =.
+                l
+                <:
+                bool)))
+      (ei_uij, ki_xj_phi
+        <:
+        (Alloc.Vec.t_Vec (Alloc.Vec.t_Vec (bool & u128) Alloc.Alloc.t_Global) Alloc.Alloc.t_Global &
+          Alloc.Vec.t_Vec (Alloc.Vec.t_Vec u128 Alloc.Alloc.t_Global) Alloc.Alloc.t_Global))
+      (fun temp_0_ j ->
+          let ei_uij, ki_xj_phi:(Alloc.Vec.t_Vec
+              (Alloc.Vec.t_Vec (bool & u128) Alloc.Alloc.t_Global) Alloc.Alloc.t_Global &
+            Alloc.Vec.t_Vec (Alloc.Vec.t_Vec u128 Alloc.Alloc.t_Global) Alloc.Alloc.t_Global) =
+            temp_0_
+          in
+          let j:usize = j in
+          if j =. i <: bool
+          then
+            ei_uij, ki_xj_phi
+            <:
             (Alloc.Vec.t_Vec (Alloc.Vec.t_Vec (bool & u128) Alloc.Alloc.t_Global)
                 Alloc.Alloc.t_Global &
               Alloc.Vec.t_Vec (Alloc.Vec.t_Vec u128 Alloc.Alloc.t_Global) Alloc.Alloc.t_Global)
-        with
-        | Core.Ops.Control_flow.ControlFlow_Break ret -> ret
-        | Core.Ops.Control_flow.ControlFlow_Continue (ei_uij, ki_xj_phi) ->
-          let tmp0, out:(iimpl_951670863_ &
-            Core.Result.t_Result
-              (Alloc.Vec.t_Vec (Alloc.Vec.t_Vec (bool & u128) Alloc.Alloc.t_Global)
-                  Alloc.Alloc.t_Global) t_Error) =
-            broadcast_first_send_second #bool
-              #u128
-              #iimpl_951670863_
-              channel
-              i
-              n
-              "flaand"
-              (Core.Ops.Deref.f_deref #(Alloc.Vec.t_Vec
-                      (Alloc.Vec.t_Vec (bool & u128) Alloc.Alloc.t_Global) Alloc.Alloc.t_Global)
-                  #FStar.Tactics.Typeclasses.solve
-                  ei_uij
-                <:
-                t_Slice (Alloc.Vec.t_Vec (bool & u128) Alloc.Alloc.t_Global))
+          else
+            Rust_primitives.Hax.Folds.fold_range (mk_usize 0)
               l
-          in
-          let channel:iimpl_951670863_ = tmp0 in
-          match
-            out
+              (fun temp_0_ temp_1_ ->
+                  let ei_uij, ki_xj_phi:(Alloc.Vec.t_Vec
+                      (Alloc.Vec.t_Vec (bool & u128) Alloc.Alloc.t_Global) Alloc.Alloc.t_Global &
+                    Alloc.Vec.t_Vec (Alloc.Vec.t_Vec u128 Alloc.Alloc.t_Global) Alloc.Alloc.t_Global
+                  ) =
+                    temp_0_
+                  in
+                  let _:usize = temp_1_ in
+                  b2t
+                  (((Alloc.Vec.impl_1__len #(Alloc.Vec.t_Vec u128 Alloc.Alloc.t_Global)
+                          #Alloc.Alloc.t_Global
+                          ki_xj_phi
+                        <:
+                        usize) =.
+                      n
+                      <:
+                      bool) &&
+                    ((Alloc.Vec.impl_1__len #(Alloc.Vec.t_Vec (bool & u128) Alloc.Alloc.t_Global)
+                          #Alloc.Alloc.t_Global
+                          ei_uij
+                        <:
+                        usize) =.
+                      n
+                      <:
+                      bool) &&
+                    ((Alloc.Vec.impl_1__len #u128 #Alloc.Alloc.t_Global phi <: usize) =. l <: bool)) /\
+                  (forall (j: usize).
+                      b2t
+                      ((mk_usize 0 <=. j <: bool) && (j <. n <: bool) &&
+                        ((Alloc.Vec.impl_1__len #(Alloc.Vec.t_Vec u128 Alloc.Alloc.t_Global)
+                              #Alloc.Alloc.t_Global
+                              ki_xj_phi
+                            <:
+                            usize) =.
+                          n
+                          <:
+                          bool)) ==>
+                      b2t
+                      ((Alloc.Vec.impl_1__len #u128
+                            #Alloc.Alloc.t_Global
+                            (ki_xj_phi.[ j ] <: Alloc.Vec.t_Vec u128 Alloc.Alloc.t_Global)
+                          <:
+                          usize) =.
+                        l
+                        <:
+                        bool)))
+              (ei_uij, ki_xj_phi
+                <:
+                (Alloc.Vec.t_Vec (Alloc.Vec.t_Vec (bool & u128) Alloc.Alloc.t_Global)
+                    Alloc.Alloc.t_Global &
+                  Alloc.Vec.t_Vec (Alloc.Vec.t_Vec u128 Alloc.Alloc.t_Global) Alloc.Alloc.t_Global))
+              (fun temp_0_ ll ->
+                  let ei_uij, ki_xj_phi:(Alloc.Vec.t_Vec
+                      (Alloc.Vec.t_Vec (bool & u128) Alloc.Alloc.t_Global) Alloc.Alloc.t_Global &
+                    Alloc.Vec.t_Vec (Alloc.Vec.t_Vec u128 Alloc.Alloc.t_Global) Alloc.Alloc.t_Global
+                  ) =
+                    temp_0_
+                  in
+                  let ll:usize = ll in
+                  let _, ki_xj:(Polytune.Data_types.t_Mac & Polytune.Data_types.t_Key) =
+                    (xshares.[ ll ] <: Polytune.Data_types.t_Share).Polytune.Data_types._1
+                      .Polytune.Data_types._0.[ j ]
+                  in
+                  let ki_xj_phi:Alloc.Vec.t_Vec (Alloc.Vec.t_Vec u128 Alloc.Alloc.t_Global)
+                    Alloc.Alloc.t_Global =
+                    Rust_primitives.Hax.Monomorphized_update_at.update_at_usize ki_xj_phi
+                      j
+                      (Rust_primitives.Hax.Monomorphized_update_at.update_at_usize (ki_xj_phi.[ j ]
+                            <:
+                            Alloc.Vec.t_Vec u128 Alloc.Alloc.t_Global)
+                          ll
+                          (hash128 ki_xj.Polytune.Data_types._0 <: u128)
+                        <:
+                        Alloc.Vec.t_Vec u128 Alloc.Alloc.t_Global)
+                  in
+                  let uij:u128 =
+                    ((hash128 (ki_xj.Polytune.Data_types._0 ^. delta.Polytune.Data_types._0 <: u128)
+                        <:
+                        u128) ^.
+                      ((ki_xj_phi.[ j ] <: Alloc.Vec.t_Vec u128 Alloc.Alloc.t_Global).[ ll ] <: u128
+                      )
+                      <:
+                      u128) ^.
+                    (phi.[ ll ] <: u128)
+                  in
+                  let ei_uij:Alloc.Vec.t_Vec (Alloc.Vec.t_Vec (bool & u128) Alloc.Alloc.t_Global)
+                    Alloc.Alloc.t_Global =
+                    Rust_primitives.Hax.Monomorphized_update_at.update_at_usize ei_uij
+                      j
+                      (Alloc.Vec.impl_1__push #(bool & u128)
+                          #Alloc.Alloc.t_Global
+                          (ei_uij.[ j ] <: Alloc.Vec.t_Vec (bool & u128) Alloc.Alloc.t_Global)
+                          ((e.[ ll ] <: bool), uij <: (bool & u128))
+                        <:
+                        Alloc.Vec.t_Vec (bool & u128) Alloc.Alloc.t_Global)
+                  in
+                  ei_uij, ki_xj_phi
+                  <:
+                  (Alloc.Vec.t_Vec (Alloc.Vec.t_Vec (bool & u128) Alloc.Alloc.t_Global)
+                      Alloc.Alloc.t_Global &
+                    Alloc.Vec.t_Vec (Alloc.Vec.t_Vec u128 Alloc.Alloc.t_Global) Alloc.Alloc.t_Global
+                  ))
             <:
-            Core.Result.t_Result
-              (Alloc.Vec.t_Vec (Alloc.Vec.t_Vec (bool & u128) Alloc.Alloc.t_Global)
-                  Alloc.Alloc.t_Global) t_Error
-          with
-          | Core.Result.Result_Ok ei_uij_k ->
-            (match
-                Rust_primitives.Hax.Folds.fold_range_return (mk_usize 0)
+            (Alloc.Vec.t_Vec (Alloc.Vec.t_Vec (bool & u128) Alloc.Alloc.t_Global)
+                Alloc.Alloc.t_Global &
+              Alloc.Vec.t_Vec (Alloc.Vec.t_Vec u128 Alloc.Alloc.t_Global) Alloc.Alloc.t_Global))
+  in
+  Core.Result.Result_Ok
+  (ki_xj_phi, ei_uij, phi
+    <:
+    (Alloc.Vec.t_Vec (Alloc.Vec.t_Vec u128 Alloc.Alloc.t_Global) Alloc.Alloc.t_Global &
+      Alloc.Vec.t_Vec (Alloc.Vec.t_Vec (bool & u128) Alloc.Alloc.t_Global) Alloc.Alloc.t_Global &
+      Alloc.Vec.t_Vec u128 Alloc.Alloc.t_Global))
+  <:
+  Core.Result.t_Result
+    (Alloc.Vec.t_Vec (Alloc.Vec.t_Vec u128 Alloc.Alloc.t_Global) Alloc.Alloc.t_Global &
+      Alloc.Vec.t_Vec (Alloc.Vec.t_Vec (bool & u128) Alloc.Alloc.t_Global) Alloc.Alloc.t_Global &
+      Alloc.Vec.t_Vec u128 Alloc.Alloc.t_Global) t_Error
+
+let flaand_2_
+      (delta: Polytune.Data_types.t_Delta)
+      (xshares rshares: t_Slice Polytune.Data_types.t_Share)
+      (i n l: usize)
+      (ki_xj_phi: Alloc.Vec.t_Vec (Alloc.Vec.t_Vec u128 Alloc.Alloc.t_Global) Alloc.Alloc.t_Global)
+      (ei_uij_k:
+          Alloc.Vec.t_Vec (Alloc.Vec.t_Vec (bool & u128) Alloc.Alloc.t_Global) Alloc.Alloc.t_Global)
+      (zshares: Alloc.Vec.t_Vec Polytune.Data_types.t_Share Alloc.Alloc.t_Global)
+      (phi: Alloc.Vec.t_Vec u128 Alloc.Alloc.t_Global)
+    : Prims.Pure
+      (Alloc.Vec.t_Vec (Alloc.Vec.t_Vec u128 Alloc.Alloc.t_Global) Alloc.Alloc.t_Global &
+        Alloc.Vec.t_Vec Polytune.Data_types.t_Share Alloc.Alloc.t_Global &
+        Core.Result.t_Result
+          (Alloc.Vec.t_Vec t_Commitment Alloc.Alloc.t_Global &
+            Alloc.Vec.t_Vec u128 Alloc.Alloc.t_Global) t_Error)
+      (requires
+        b2t ((Alloc.Vec.impl_1__len #u128 #Alloc.Alloc.t_Global phi <: usize) >=. l <: bool) /\
+        b2t ((Core.Slice.impl__len #Polytune.Data_types.t_Share rshares <: usize) >=. l <: bool) /\
+        (forall (ll: usize).
+            b2t
+            ((mk_usize 0 <=. ll <: bool) && (ll <. l <: bool) &&
+              ((Core.Slice.impl__len #Polytune.Data_types.t_Share rshares <: usize) >=. l <: bool)) ==>
+            b2t
+            ((Alloc.Vec.impl_1__len #(Polytune.Data_types.t_Mac & Polytune.Data_types.t_Key)
+                  #Alloc.Alloc.t_Global
+                  (rshares.[ ll ] <: Polytune.Data_types.t_Share).Polytune.Data_types._1
+                    .Polytune.Data_types._0
+                <:
+                usize) >=.
+              n
+              <:
+              bool)) /\
+        (b2t
+        ((Alloc.Vec.impl_1__len #Polytune.Data_types.t_Share #Alloc.Alloc.t_Global zshares <: usize) >=.
+          l
+          <:
+          bool) /\
+        (forall (ll: usize).
+            b2t
+            ((mk_usize 0 <=. ll <: bool) && (ll <. l <: bool) &&
+              ((Alloc.Vec.impl_1__len #Polytune.Data_types.t_Share #Alloc.Alloc.t_Global zshares
+                  <:
+                  usize) >=.
+                l
+                <:
+                bool)) ==>
+            b2t
+            ((Alloc.Vec.impl_1__len #(Polytune.Data_types.t_Mac & Polytune.Data_types.t_Key)
+                  #Alloc.Alloc.t_Global
+                  (zshares.[ ll ] <: Polytune.Data_types.t_Share).Polytune.Data_types._1
+                    .Polytune.Data_types._0
+                <:
+                usize) >=.
+              n
+              <:
+              bool)) /\
+        (b2t ((Core.Slice.impl__len #Polytune.Data_types.t_Share xshares <: usize) >=. l <: bool) /\
+        (forall (ll: usize).
+            b2t
+            ((mk_usize 0 <=. ll <: bool) && (ll <. l <: bool) &&
+              ((Core.Slice.impl__len #Polytune.Data_types.t_Share xshares <: usize) >=. l <: bool)) ==>
+            b2t
+            ((Alloc.Vec.impl_1__len #(Polytune.Data_types.t_Mac & Polytune.Data_types.t_Key)
+                  #Alloc.Alloc.t_Global
+                  (xshares.[ ll ] <: Polytune.Data_types.t_Share).Polytune.Data_types._1
+                    .Polytune.Data_types._0
+                <:
+                usize) >=.
+              n
+              <:
+              bool)))) /\
+        (b2t
+        ((Alloc.Vec.impl_1__len #(Alloc.Vec.t_Vec (bool & u128) Alloc.Alloc.t_Global)
+              #Alloc.Alloc.t_Global
+              ei_uij_k
+            <:
+            usize) >=.
+          n
+          <:
+          bool) /\
+        (forall (j: usize).
+            b2t
+            ((mk_usize 0 <=. j <: bool) && (j <. n <: bool) &&
+              ((Alloc.Vec.impl_1__len #(Alloc.Vec.t_Vec (bool & u128) Alloc.Alloc.t_Global)
+                    #Alloc.Alloc.t_Global
+                    ei_uij_k
+                  <:
+                  usize) >=.
+                n
+                <:
+                bool)) ==>
+            b2t
+            ((Alloc.Vec.impl_1__len #(bool & u128)
+                  #Alloc.Alloc.t_Global
+                  (ei_uij_k.[ j ] <: Alloc.Vec.t_Vec (bool & u128) Alloc.Alloc.t_Global)
+                <:
+                usize) >=.
+              l
+              <:
+              bool)) /\
+        (b2t
+        ((Alloc.Vec.impl_1__len #(Alloc.Vec.t_Vec u128 Alloc.Alloc.t_Global)
+              #Alloc.Alloc.t_Global
+              ki_xj_phi
+            <:
+            usize) >=.
+          n
+          <:
+          bool) /\
+        (forall (j: usize).
+            b2t
+            ((mk_usize 0 <=. j <: bool) && (j <. n <: bool) &&
+              ((Alloc.Vec.impl_1__len #(Alloc.Vec.t_Vec u128 Alloc.Alloc.t_Global)
+                    #Alloc.Alloc.t_Global
+                    ki_xj_phi
+                  <:
+                  usize) >=.
+                n
+                <:
+                bool)) ==>
+            b2t
+            ((Alloc.Vec.impl_1__len #u128
+                  #Alloc.Alloc.t_Global
+                  (ki_xj_phi.[ j ] <: Alloc.Vec.t_Vec u128 Alloc.Alloc.t_Global)
+                <:
+                usize) >=.
+              l
+              <:
+              bool)))))
+      (fun _ -> Prims.l_True) =
+  let ki_xj_phi, zshares:(Alloc.Vec.t_Vec (Alloc.Vec.t_Vec u128 Alloc.Alloc.t_Global)
+      Alloc.Alloc.t_Global &
+    Alloc.Vec.t_Vec Polytune.Data_types.t_Share Alloc.Alloc.t_Global) =
+    Rust_primitives.Hax.Folds.fold_range (mk_usize 0)
+      n
+      (fun temp_0_ temp_1_ ->
+          let ki_xj_phi, zshares:(Alloc.Vec.t_Vec (Alloc.Vec.t_Vec u128 Alloc.Alloc.t_Global)
+              Alloc.Alloc.t_Global &
+            Alloc.Vec.t_Vec Polytune.Data_types.t_Share Alloc.Alloc.t_Global) =
+            temp_0_
+          in
+          let _:usize = temp_1_ in
+          b2t
+          ((Alloc.Vec.impl_1__len #(Alloc.Vec.t_Vec u128 Alloc.Alloc.t_Global)
+                #Alloc.Alloc.t_Global
+                ki_xj_phi
+              <:
+              usize) >=.
+            n
+            <:
+            bool) /\
+          (forall (j: usize).
+              b2t
+              ((mk_usize 0 <=. j <: bool) && (j <. n <: bool) &&
+                ((Alloc.Vec.impl_1__len #(Alloc.Vec.t_Vec u128 Alloc.Alloc.t_Global)
+                      #Alloc.Alloc.t_Global
+                      ki_xj_phi
+                    <:
+                    usize) >=.
                   n
-                  (fun temp_0_ temp_1_ ->
-                      let ki_xj_phi, zshares:(Alloc.Vec.t_Vec
-                          (Alloc.Vec.t_Vec u128 Alloc.Alloc.t_Global) Alloc.Alloc.t_Global &
-                        Alloc.Vec.t_Vec Polytune.Data_types.t_Share Alloc.Alloc.t_Global) =
-                        temp_0_
-                      in
-                      let _:usize = temp_1_ in
-                      true)
-                  (ki_xj_phi, zshares
+                  <:
+                  bool)) ==>
+              b2t
+              ((Alloc.Vec.impl_1__len #u128
+                    #Alloc.Alloc.t_Global
+                    (ki_xj_phi.[ j ] <: Alloc.Vec.t_Vec u128 Alloc.Alloc.t_Global)
+                  <:
+                  usize) >=.
+                l
+                <:
+                bool)) /\
+          b2t
+          ((Alloc.Vec.impl_1__len #Polytune.Data_types.t_Share #Alloc.Alloc.t_Global zshares
+              <:
+              usize) >=.
+            l
+            <:
+            bool) /\
+          (forall (ll: usize).
+              b2t
+              ((mk_usize 0 <=. ll <: bool) && (ll <. l <: bool) &&
+                ((Alloc.Vec.impl_1__len #Polytune.Data_types.t_Share #Alloc.Alloc.t_Global zshares
+                    <:
+                    usize) >=.
+                  l
+                  <:
+                  bool)) ==>
+              b2t
+              ((Alloc.Vec.impl_1__len #(Polytune.Data_types.t_Mac & Polytune.Data_types.t_Key)
+                    #Alloc.Alloc.t_Global
+                    (zshares.[ ll ] <: Polytune.Data_types.t_Share).Polytune.Data_types._1
+                      .Polytune.Data_types._0
+                  <:
+                  usize) >=.
+                n
+                <:
+                bool)))
+      (ki_xj_phi, zshares
+        <:
+        (Alloc.Vec.t_Vec (Alloc.Vec.t_Vec u128 Alloc.Alloc.t_Global) Alloc.Alloc.t_Global &
+          Alloc.Vec.t_Vec Polytune.Data_types.t_Share Alloc.Alloc.t_Global))
+      (fun temp_0_ j ->
+          let ki_xj_phi, zshares:(Alloc.Vec.t_Vec (Alloc.Vec.t_Vec u128 Alloc.Alloc.t_Global)
+              Alloc.Alloc.t_Global &
+            Alloc.Vec.t_Vec Polytune.Data_types.t_Share Alloc.Alloc.t_Global) =
+            temp_0_
+          in
+          let j:usize = j in
+          if j =. i <: bool
+          then
+            ki_xj_phi, zshares
+            <:
+            (Alloc.Vec.t_Vec (Alloc.Vec.t_Vec u128 Alloc.Alloc.t_Global) Alloc.Alloc.t_Global &
+              Alloc.Vec.t_Vec Polytune.Data_types.t_Share Alloc.Alloc.t_Global)
+          else
+            Rust_primitives.Hax.Folds.fold_range (mk_usize 0)
+              l
+              (fun temp_0_ temp_1_ ->
+                  let ki_xj_phi, zshares:(Alloc.Vec.t_Vec
+                      (Alloc.Vec.t_Vec u128 Alloc.Alloc.t_Global) Alloc.Alloc.t_Global &
+                    Alloc.Vec.t_Vec Polytune.Data_types.t_Share Alloc.Alloc.t_Global) =
+                    temp_0_
+                  in
+                  let _:usize = temp_1_ in
+                  b2t
+                  ((Alloc.Vec.impl_1__len #(Alloc.Vec.t_Vec u128 Alloc.Alloc.t_Global)
+                        #Alloc.Alloc.t_Global
+                        ki_xj_phi
+                      <:
+                      usize) >=.
+                    n
+                    <:
+                    bool) /\
+                  (forall (j: usize).
+                      b2t
+                      ((mk_usize 0 <=. j <: bool) && (j <. n <: bool) &&
+                        ((Alloc.Vec.impl_1__len #(Alloc.Vec.t_Vec u128 Alloc.Alloc.t_Global)
+                              #Alloc.Alloc.t_Global
+                              ki_xj_phi
+                            <:
+                            usize) >=.
+                          n
+                          <:
+                          bool)) ==>
+                      b2t
+                      ((Alloc.Vec.impl_1__len #u128
+                            #Alloc.Alloc.t_Global
+                            (ki_xj_phi.[ j ] <: Alloc.Vec.t_Vec u128 Alloc.Alloc.t_Global)
+                          <:
+                          usize) >=.
+                        l
+                        <:
+                        bool)) /\
+                  b2t
+                  ((Alloc.Vec.impl_1__len #Polytune.Data_types.t_Share #Alloc.Alloc.t_Global zshares
+                      <:
+                      usize) >=.
+                    l
+                    <:
+                    bool) /\
+                  (forall (ll: usize).
+                      b2t
+                      ((mk_usize 0 <=. ll <: bool) && (ll <. l <: bool) &&
+                        ((Alloc.Vec.impl_1__len #Polytune.Data_types.t_Share
+                              #Alloc.Alloc.t_Global
+                              zshares
+                            <:
+                            usize) >=.
+                          l
+                          <:
+                          bool)) ==>
+                      b2t
+                      ((Alloc.Vec.impl_1__len #(Polytune.Data_types.t_Mac &
+                              Polytune.Data_types.t_Key)
+                            #Alloc.Alloc.t_Global
+                            (zshares.[ ll ] <: Polytune.Data_types.t_Share).Polytune.Data_types._1
+                              .Polytune.Data_types._0
+                          <:
+                          usize) >=.
+                        n
+                        <:
+                        bool)))
+              (ki_xj_phi, zshares
+                <:
+                (Alloc.Vec.t_Vec (Alloc.Vec.t_Vec u128 Alloc.Alloc.t_Global) Alloc.Alloc.t_Global &
+                  Alloc.Vec.t_Vec Polytune.Data_types.t_Share Alloc.Alloc.t_Global))
+              (fun temp_0_ ll ->
+                  let ki_xj_phi, zshares:(Alloc.Vec.t_Vec
+                      (Alloc.Vec.t_Vec u128 Alloc.Alloc.t_Global) Alloc.Alloc.t_Global &
+                    Alloc.Vec.t_Vec Polytune.Data_types.t_Share Alloc.Alloc.t_Global) =
+                    temp_0_
+                  in
+                  let ll:usize = ll in
+                  let mi_xj, _:(Polytune.Data_types.t_Mac & Polytune.Data_types.t_Key) =
+                    (xshares.[ ll ] <: Polytune.Data_types.t_Share).Polytune.Data_types._1
+                      .Polytune.Data_types._0.[ j ]
+                  in
+                  let ki_xj_phi:Alloc.Vec.t_Vec (Alloc.Vec.t_Vec u128 Alloc.Alloc.t_Global)
+                    Alloc.Alloc.t_Global =
+                    Rust_primitives.Hax.Monomorphized_update_at.update_at_usize ki_xj_phi
+                      j
+                      (Rust_primitives.Hax.Monomorphized_update_at.update_at_usize (ki_xj_phi.[ j ]
+                            <:
+                            Alloc.Vec.t_Vec u128 Alloc.Alloc.t_Global)
+                          ll
+                          ((((ki_xj_phi.[ j ] <: Alloc.Vec.t_Vec u128 Alloc.Alloc.t_Global).[ ll ]
+                                <:
+                                u128) ^.
+                              (hash128 mi_xj.Polytune.Data_types._0 <: u128)
+                              <:
+                              u128) ^.
+                            ((cast ((xshares.[ ll ] <: Polytune.Data_types.t_Share)
+                                      .Polytune.Data_types._0
+                                    <:
+                                    bool)
+                                <:
+                                u128) *!
+                              ((ei_uij_k.[ j ] <: Alloc.Vec.t_Vec (bool & u128) Alloc.Alloc.t_Global
+                                ).[ ll ]
+                                <:
+                                (bool & u128))
+                                ._2
+                              <:
+                              u128)
+                            <:
+                            u128)
+                        <:
+                        Alloc.Vec.t_Vec u128 Alloc.Alloc.t_Global)
+                  in
+                  let mac, key:(Polytune.Data_types.t_Mac & Polytune.Data_types.t_Key) =
+                    (rshares.[ ll ] <: Polytune.Data_types.t_Share).Polytune.Data_types._1
+                      .Polytune.Data_types._0.[ j ]
+                  in
+                  if
+                    ((ei_uij_k.[ j ] <: Alloc.Vec.t_Vec (bool & u128) Alloc.Alloc.t_Global).[ ll ] <: (bool & u128))
+                      ._1
+                  then
+                    let zshares:Alloc.Vec.t_Vec Polytune.Data_types.t_Share Alloc.Alloc.t_Global =
+                      Rust_primitives.Hax.Monomorphized_update_at.update_at_usize zshares
+                        ll
+                        ({
+                            (zshares.[ ll ] <: Polytune.Data_types.t_Share) with
+                            Polytune.Data_types._1
+                            =
+                            {
+                              (zshares.[ ll ] <: Polytune.Data_types.t_Share).Polytune.Data_types._1 with
+                              Polytune.Data_types._0
+                              =
+                              Rust_primitives.Hax.Monomorphized_update_at.update_at_usize (zshares.[
+                                    ll ]
+                                  <:
+                                  Polytune.Data_types.t_Share)
+                                  .Polytune.Data_types._1
+                                  .Polytune.Data_types._0
+                                j
+                                (mac,
+                                  (Polytune.Data_types.Key
+                                    (key.Polytune.Data_types._0 ^. delta.Polytune.Data_types._0
+                                      <:
+                                      u128)
+                                    <:
+                                    Polytune.Data_types.t_Key)
+                                  <:
+                                  (Polytune.Data_types.t_Mac & Polytune.Data_types.t_Key))
+                              <:
+                              Alloc.Vec.t_Vec
+                                (Polytune.Data_types.t_Mac & Polytune.Data_types.t_Key)
+                                Alloc.Alloc.t_Global
+                            }
+                            <:
+                            Polytune.Data_types.t_Auth
+                          }
+                          <:
+                          Polytune.Data_types.t_Share)
+                    in
+                    ki_xj_phi, zshares
+                    <:
+                    (Alloc.Vec.t_Vec (Alloc.Vec.t_Vec u128 Alloc.Alloc.t_Global)
+                        Alloc.Alloc.t_Global &
+                      Alloc.Vec.t_Vec Polytune.Data_types.t_Share Alloc.Alloc.t_Global)
+                  else
+                    let zshares:Alloc.Vec.t_Vec Polytune.Data_types.t_Share Alloc.Alloc.t_Global =
+                      Rust_primitives.Hax.Monomorphized_update_at.update_at_usize zshares
+                        ll
+                        ({
+                            (zshares.[ ll ] <: Polytune.Data_types.t_Share) with
+                            Polytune.Data_types._1
+                            =
+                            {
+                              (zshares.[ ll ] <: Polytune.Data_types.t_Share).Polytune.Data_types._1 with
+                              Polytune.Data_types._0
+                              =
+                              Rust_primitives.Hax.Monomorphized_update_at.update_at_usize (zshares.[
+                                    ll ]
+                                  <:
+                                  Polytune.Data_types.t_Share)
+                                  .Polytune.Data_types._1
+                                  .Polytune.Data_types._0
+                                j
+                                (mac, key <: (Polytune.Data_types.t_Mac & Polytune.Data_types.t_Key)
+                                )
+                              <:
+                              Alloc.Vec.t_Vec
+                                (Polytune.Data_types.t_Mac & Polytune.Data_types.t_Key)
+                                Alloc.Alloc.t_Global
+                            }
+                            <:
+                            Polytune.Data_types.t_Auth
+                          }
+                          <:
+                          Polytune.Data_types.t_Share)
+                    in
+                    ki_xj_phi, zshares
                     <:
                     (Alloc.Vec.t_Vec (Alloc.Vec.t_Vec u128 Alloc.Alloc.t_Global)
                         Alloc.Alloc.t_Global &
                       Alloc.Vec.t_Vec Polytune.Data_types.t_Share Alloc.Alloc.t_Global))
-                  (fun temp_0_ j ->
-                      let ki_xj_phi, zshares:(Alloc.Vec.t_Vec
-                          (Alloc.Vec.t_Vec u128 Alloc.Alloc.t_Global) Alloc.Alloc.t_Global &
-                        Alloc.Vec.t_Vec Polytune.Data_types.t_Share Alloc.Alloc.t_Global) =
-                        temp_0_
-                      in
-                      let j:usize = j in
-                      if j =. i <: bool
-                      then
-                        Core.Ops.Control_flow.ControlFlow_Continue
-                        (ki_xj_phi, zshares
-                          <:
-                          (Alloc.Vec.t_Vec (Alloc.Vec.t_Vec u128 Alloc.Alloc.t_Global)
-                              Alloc.Alloc.t_Global &
-                            Alloc.Vec.t_Vec Polytune.Data_types.t_Share Alloc.Alloc.t_Global))
-                        <:
-                        Core.Ops.Control_flow.t_ControlFlow
-                          (Core.Ops.Control_flow.t_ControlFlow
-                              (iimpl_951670863_ &
-                                Core.Result.t_Result
-                                  (Alloc.Vec.t_Vec Polytune.Data_types.t_Share Alloc.Alloc.t_Global)
-                                  t_Error)
-                              (Prims.unit &
-                                (Alloc.Vec.t_Vec (Alloc.Vec.t_Vec u128 Alloc.Alloc.t_Global)
-                                    Alloc.Alloc.t_Global &
-                                  Alloc.Vec.t_Vec Polytune.Data_types.t_Share Alloc.Alloc.t_Global))
-                          )
-                          (Alloc.Vec.t_Vec (Alloc.Vec.t_Vec u128 Alloc.Alloc.t_Global)
-                              Alloc.Alloc.t_Global &
-                            Alloc.Vec.t_Vec Polytune.Data_types.t_Share Alloc.Alloc.t_Global)
-                      else
-                        match
-                          Rust_primitives.Hax.Folds.fold_return (Core.Iter.Traits.Collect.f_into_iter
-                                #(Core.Iter.Adapters.Take.t_Take
-                                  (Core.Iter.Adapters.Enumerate.t_Enumerate
-                                    (Core.Slice.Iter.t_Iter Polytune.Data_types.t_Share)))
-                                #FStar.Tactics.Typeclasses.solve
-                                (Core.Iter.Traits.Iterator.f_take #(Core.Iter.Adapters.Enumerate.t_Enumerate
-                                      (Core.Slice.Iter.t_Iter Polytune.Data_types.t_Share))
-                                    #FStar.Tactics.Typeclasses.solve
-                                    (Core.Iter.Traits.Iterator.f_enumerate #(Core.Slice.Iter.t_Iter
-                                          Polytune.Data_types.t_Share)
-                                        #FStar.Tactics.Typeclasses.solve
-                                        (Core.Slice.impl__iter #Polytune.Data_types.t_Share xshares
-                                          <:
-                                          Core.Slice.Iter.t_Iter Polytune.Data_types.t_Share)
-                                      <:
-                                      Core.Iter.Adapters.Enumerate.t_Enumerate
-                                      (Core.Slice.Iter.t_Iter Polytune.Data_types.t_Share))
-                                    l
-                                  <:
-                                  Core.Iter.Adapters.Take.t_Take
-                                  (Core.Iter.Adapters.Enumerate.t_Enumerate
-                                    (Core.Slice.Iter.t_Iter Polytune.Data_types.t_Share)))
-                              <:
-                              Core.Iter.Adapters.Take.t_Take
-                              (Core.Iter.Adapters.Enumerate.t_Enumerate
-                                (Core.Slice.Iter.t_Iter Polytune.Data_types.t_Share)))
-                            (ki_xj_phi, zshares
-                              <:
-                              (Alloc.Vec.t_Vec (Alloc.Vec.t_Vec u128 Alloc.Alloc.t_Global)
-                                  Alloc.Alloc.t_Global &
-                                Alloc.Vec.t_Vec Polytune.Data_types.t_Share Alloc.Alloc.t_Global))
-                            (fun temp_0_ temp_1_ ->
-                                let ki_xj_phi, zshares:(Alloc.Vec.t_Vec
-                                    (Alloc.Vec.t_Vec u128 Alloc.Alloc.t_Global) Alloc.Alloc.t_Global &
-                                  Alloc.Vec.t_Vec Polytune.Data_types.t_Share Alloc.Alloc.t_Global)
-                                =
-                                  temp_0_
-                                in
-                                let ll, xbit:(usize & Polytune.Data_types.t_Share) = temp_1_ in
-                                let mi_xj, _:(Polytune.Data_types.t_Mac & Polytune.Data_types.t_Key)
-                                =
-                                  (xshares.[ ll ] <: Polytune.Data_types.t_Share)
-                                    .Polytune.Data_types._1
-                                    .Polytune.Data_types._0.[ j ]
-                                in
-                                match
-                                  hash128 mi_xj.Polytune.Data_types._0
-                                  <:
-                                  Core.Result.t_Result u128 t_Error
-                                with
-                                | Core.Result.Result_Ok hoist16 ->
-                                  let ki_xj_phi:Alloc.Vec.t_Vec
-                                    (Alloc.Vec.t_Vec u128 Alloc.Alloc.t_Global) Alloc.Alloc.t_Global
-                                  =
-                                    Rust_primitives.Hax.Monomorphized_update_at.update_at_usize ki_xj_phi
-                                      j
-                                      (Rust_primitives.Hax.Monomorphized_update_at.update_at_usize (ki_xj_phi.[
-                                              j ]
-                                            <:
-                                            Alloc.Vec.t_Vec u128 Alloc.Alloc.t_Global)
-                                          ll
-                                          ((((ki_xj_phi.[ j ]
-                                                  <:
-                                                  Alloc.Vec.t_Vec u128 Alloc.Alloc.t_Global).[ ll ]
-                                                <:
-                                                u128) ^.
-                                              hoist16
-                                              <:
-                                              u128) ^.
-                                            ((cast (xbit.Polytune.Data_types._0 <: bool) <: u128) *!
-                                              ((ei_uij_k.[ j ]
-                                                  <:
-                                                  Alloc.Vec.t_Vec (bool & u128) Alloc.Alloc.t_Global
-                                                ).[ ll ]
-                                                <:
-                                                (bool & u128))
-                                                ._2
-                                              <:
-                                              u128)
-                                            <:
-                                            u128)
-                                        <:
-                                        Alloc.Vec.t_Vec u128 Alloc.Alloc.t_Global)
-                                  in
-                                  let mac, key:(Polytune.Data_types.t_Mac &
-                                    Polytune.Data_types.t_Key) =
-                                    (rshares.[ ll ] <: Polytune.Data_types.t_Share)
-                                      .Polytune.Data_types._1
-                                      .Polytune.Data_types._0.[ j ]
-                                  in
-                                  if
-                                    ((ei_uij_k.[ j ]
-                                        <:
-                                        Alloc.Vec.t_Vec (bool & u128) Alloc.Alloc.t_Global).[ ll ] <: (bool & u128))
-                                      ._1
-                                  then
-                                    let zshares:Alloc.Vec.t_Vec Polytune.Data_types.t_Share
-                                      Alloc.Alloc.t_Global =
-                                      Rust_primitives.Hax.Monomorphized_update_at.update_at_usize zshares
-                                        ll
-                                        ({
-                                            (zshares.[ ll ] <: Polytune.Data_types.t_Share) with
-                                            Polytune.Data_types._1
-                                            =
-                                            {
-                                              (zshares.[ ll ] <: Polytune.Data_types.t_Share)
-                                                .Polytune.Data_types._1 with
-                                              Polytune.Data_types._0
-                                              =
-                                              Rust_primitives.Hax.Monomorphized_update_at.update_at_usize
-                                                (zshares.[ ll ] <: Polytune.Data_types.t_Share)
-                                                  .Polytune.Data_types._1
-                                                  .Polytune.Data_types._0
-                                                j
-                                                (mac,
-                                                  (Polytune.Data_types.Key
-                                                    (key.Polytune.Data_types._0 ^.
-                                                      delta.Polytune.Data_types._0
-                                                      <:
-                                                      u128)
-                                                    <:
-                                                    Polytune.Data_types.t_Key)
-                                                  <:
-                                                  (Polytune.Data_types.t_Mac &
-                                                    Polytune.Data_types.t_Key))
-                                              <:
-                                              Alloc.Vec.t_Vec
-                                                (Polytune.Data_types.t_Mac &
-                                                  Polytune.Data_types.t_Key) Alloc.Alloc.t_Global
-                                            }
-                                            <:
-                                            Polytune.Data_types.t_Auth
-                                          }
-                                          <:
-                                          Polytune.Data_types.t_Share)
-                                    in
-                                    Core.Ops.Control_flow.ControlFlow_Continue
-                                    (ki_xj_phi, zshares
-                                      <:
-                                      (Alloc.Vec.t_Vec (Alloc.Vec.t_Vec u128 Alloc.Alloc.t_Global)
-                                          Alloc.Alloc.t_Global &
-                                        Alloc.Vec.t_Vec Polytune.Data_types.t_Share
-                                          Alloc.Alloc.t_Global))
-                                    <:
-                                    Core.Ops.Control_flow.t_ControlFlow
-                                      (Core.Ops.Control_flow.t_ControlFlow
-                                          (iimpl_951670863_ &
-                                            Core.Result.t_Result
-                                              (Alloc.Vec.t_Vec Polytune.Data_types.t_Share
-                                                  Alloc.Alloc.t_Global) t_Error)
-                                          (Prims.unit &
-                                            (Alloc.Vec.t_Vec
-                                                (Alloc.Vec.t_Vec u128 Alloc.Alloc.t_Global)
-                                                Alloc.Alloc.t_Global &
-                                              Alloc.Vec.t_Vec Polytune.Data_types.t_Share
-                                                Alloc.Alloc.t_Global)))
-                                      (Alloc.Vec.t_Vec (Alloc.Vec.t_Vec u128 Alloc.Alloc.t_Global)
-                                          Alloc.Alloc.t_Global &
-                                        Alloc.Vec.t_Vec Polytune.Data_types.t_Share
-                                          Alloc.Alloc.t_Global)
-                                  else
-                                    let zshares:Alloc.Vec.t_Vec Polytune.Data_types.t_Share
-                                      Alloc.Alloc.t_Global =
-                                      Rust_primitives.Hax.Monomorphized_update_at.update_at_usize zshares
-                                        ll
-                                        ({
-                                            (zshares.[ ll ] <: Polytune.Data_types.t_Share) with
-                                            Polytune.Data_types._1
-                                            =
-                                            {
-                                              (zshares.[ ll ] <: Polytune.Data_types.t_Share)
-                                                .Polytune.Data_types._1 with
-                                              Polytune.Data_types._0
-                                              =
-                                              Rust_primitives.Hax.Monomorphized_update_at.update_at_usize
-                                                (zshares.[ ll ] <: Polytune.Data_types.t_Share)
-                                                  .Polytune.Data_types._1
-                                                  .Polytune.Data_types._0
-                                                j
-                                                (mac, key
-                                                  <:
-                                                  (Polytune.Data_types.t_Mac &
-                                                    Polytune.Data_types.t_Key))
-                                              <:
-                                              Alloc.Vec.t_Vec
-                                                (Polytune.Data_types.t_Mac &
-                                                  Polytune.Data_types.t_Key) Alloc.Alloc.t_Global
-                                            }
-                                            <:
-                                            Polytune.Data_types.t_Auth
-                                          }
-                                          <:
-                                          Polytune.Data_types.t_Share)
-                                    in
-                                    Core.Ops.Control_flow.ControlFlow_Continue
-                                    (ki_xj_phi, zshares
-                                      <:
-                                      (Alloc.Vec.t_Vec (Alloc.Vec.t_Vec u128 Alloc.Alloc.t_Global)
-                                          Alloc.Alloc.t_Global &
-                                        Alloc.Vec.t_Vec Polytune.Data_types.t_Share
-                                          Alloc.Alloc.t_Global))
-                                    <:
-                                    Core.Ops.Control_flow.t_ControlFlow
-                                      (Core.Ops.Control_flow.t_ControlFlow
-                                          (iimpl_951670863_ &
-                                            Core.Result.t_Result
-                                              (Alloc.Vec.t_Vec Polytune.Data_types.t_Share
-                                                  Alloc.Alloc.t_Global) t_Error)
-                                          (Prims.unit &
-                                            (Alloc.Vec.t_Vec
-                                                (Alloc.Vec.t_Vec u128 Alloc.Alloc.t_Global)
-                                                Alloc.Alloc.t_Global &
-                                              Alloc.Vec.t_Vec Polytune.Data_types.t_Share
-                                                Alloc.Alloc.t_Global)))
-                                      (Alloc.Vec.t_Vec (Alloc.Vec.t_Vec u128 Alloc.Alloc.t_Global)
-                                          Alloc.Alloc.t_Global &
-                                        Alloc.Vec.t_Vec Polytune.Data_types.t_Share
-                                          Alloc.Alloc.t_Global)
-                                | Core.Result.Result_Err err ->
-                                  Core.Ops.Control_flow.ControlFlow_Break
-                                  (Core.Ops.Control_flow.ControlFlow_Break
-                                    (channel,
-                                      (Core.Result.Result_Err err
-                                        <:
-                                        Core.Result.t_Result
-                                          (Alloc.Vec.t_Vec Polytune.Data_types.t_Share
-                                              Alloc.Alloc.t_Global) t_Error)
-                                      <:
-                                      (iimpl_951670863_ &
-                                        Core.Result.t_Result
-                                          (Alloc.Vec.t_Vec Polytune.Data_types.t_Share
-                                              Alloc.Alloc.t_Global) t_Error))
-                                    <:
-                                    Core.Ops.Control_flow.t_ControlFlow
-                                      (iimpl_951670863_ &
-                                        Core.Result.t_Result
-                                          (Alloc.Vec.t_Vec Polytune.Data_types.t_Share
-                                              Alloc.Alloc.t_Global) t_Error)
-                                      (Prims.unit &
-                                        (Alloc.Vec.t_Vec (Alloc.Vec.t_Vec u128 Alloc.Alloc.t_Global)
-                                            Alloc.Alloc.t_Global &
-                                          Alloc.Vec.t_Vec Polytune.Data_types.t_Share
-                                            Alloc.Alloc.t_Global)))
-                                  <:
-                                  Core.Ops.Control_flow.t_ControlFlow
-                                    (Core.Ops.Control_flow.t_ControlFlow
-                                        (iimpl_951670863_ &
-                                          Core.Result.t_Result
-                                            (Alloc.Vec.t_Vec Polytune.Data_types.t_Share
-                                                Alloc.Alloc.t_Global) t_Error)
-                                        (Prims.unit &
-                                          (Alloc.Vec.t_Vec
-                                              (Alloc.Vec.t_Vec u128 Alloc.Alloc.t_Global)
-                                              Alloc.Alloc.t_Global &
-                                            Alloc.Vec.t_Vec Polytune.Data_types.t_Share
-                                              Alloc.Alloc.t_Global)))
-                                    (Alloc.Vec.t_Vec (Alloc.Vec.t_Vec u128 Alloc.Alloc.t_Global)
-                                        Alloc.Alloc.t_Global &
-                                      Alloc.Vec.t_Vec Polytune.Data_types.t_Share
-                                        Alloc.Alloc.t_Global))
-                          <:
-                          Core.Ops.Control_flow.t_ControlFlow
-                            (iimpl_951670863_ &
-                              Core.Result.t_Result
-                                (Alloc.Vec.t_Vec Polytune.Data_types.t_Share Alloc.Alloc.t_Global)
-                                t_Error)
-                            (Alloc.Vec.t_Vec (Alloc.Vec.t_Vec u128 Alloc.Alloc.t_Global)
-                                Alloc.Alloc.t_Global &
-                              Alloc.Vec.t_Vec Polytune.Data_types.t_Share Alloc.Alloc.t_Global)
-                        with
-                        | Core.Ops.Control_flow.ControlFlow_Break ret ->
-                          Core.Ops.Control_flow.ControlFlow_Break
-                          (Core.Ops.Control_flow.ControlFlow_Break ret
-                            <:
-                            Core.Ops.Control_flow.t_ControlFlow
-                              (iimpl_951670863_ &
-                                Core.Result.t_Result
-                                  (Alloc.Vec.t_Vec Polytune.Data_types.t_Share Alloc.Alloc.t_Global)
-                                  t_Error)
-                              (Prims.unit &
-                                (Alloc.Vec.t_Vec (Alloc.Vec.t_Vec u128 Alloc.Alloc.t_Global)
-                                    Alloc.Alloc.t_Global &
-                                  Alloc.Vec.t_Vec Polytune.Data_types.t_Share Alloc.Alloc.t_Global))
-                          )
-                          <:
-                          Core.Ops.Control_flow.t_ControlFlow
-                            (Core.Ops.Control_flow.t_ControlFlow
-                                (iimpl_951670863_ &
-                                  Core.Result.t_Result
-                                    (Alloc.Vec.t_Vec Polytune.Data_types.t_Share
-                                        Alloc.Alloc.t_Global) t_Error)
-                                (Prims.unit &
-                                  (Alloc.Vec.t_Vec (Alloc.Vec.t_Vec u128 Alloc.Alloc.t_Global)
-                                      Alloc.Alloc.t_Global &
-                                    Alloc.Vec.t_Vec Polytune.Data_types.t_Share Alloc.Alloc.t_Global
-                                  )))
-                            (Alloc.Vec.t_Vec (Alloc.Vec.t_Vec u128 Alloc.Alloc.t_Global)
-                                Alloc.Alloc.t_Global &
-                              Alloc.Vec.t_Vec Polytune.Data_types.t_Share Alloc.Alloc.t_Global)
-                        | Core.Ops.Control_flow.ControlFlow_Continue loop_res ->
-                          Core.Ops.Control_flow.ControlFlow_Continue loop_res
-                          <:
-                          Core.Ops.Control_flow.t_ControlFlow
-                            (Core.Ops.Control_flow.t_ControlFlow
-                                (iimpl_951670863_ &
-                                  Core.Result.t_Result
-                                    (Alloc.Vec.t_Vec Polytune.Data_types.t_Share
-                                        Alloc.Alloc.t_Global) t_Error)
-                                (Prims.unit &
-                                  (Alloc.Vec.t_Vec (Alloc.Vec.t_Vec u128 Alloc.Alloc.t_Global)
-                                      Alloc.Alloc.t_Global &
-                                    Alloc.Vec.t_Vec Polytune.Data_types.t_Share Alloc.Alloc.t_Global
-                                  )))
-                            (Alloc.Vec.t_Vec (Alloc.Vec.t_Vec u128 Alloc.Alloc.t_Global)
-                                Alloc.Alloc.t_Global &
-                              Alloc.Vec.t_Vec Polytune.Data_types.t_Share Alloc.Alloc.t_Global))
+            <:
+            (Alloc.Vec.t_Vec (Alloc.Vec.t_Vec u128 Alloc.Alloc.t_Global) Alloc.Alloc.t_Global &
+              Alloc.Vec.t_Vec Polytune.Data_types.t_Share Alloc.Alloc.t_Global))
+  in
+  let hi:Alloc.Vec.t_Vec u128 Alloc.Alloc.t_Global = Alloc.Vec.from_elem #u128 (mk_u128 0) l in
+  let commhi:Alloc.Vec.t_Vec t_Commitment Alloc.Alloc.t_Global =
+    Alloc.Vec.impl__with_capacity #t_Commitment l
+  in
+  let commhi, hi:(Alloc.Vec.t_Vec t_Commitment Alloc.Alloc.t_Global &
+    Alloc.Vec.t_Vec u128 Alloc.Alloc.t_Global) =
+    Rust_primitives.Hax.Folds.fold_range (mk_usize 0)
+      l
+      (fun temp_0_ ll ->
+          let commhi, hi:(Alloc.Vec.t_Vec t_Commitment Alloc.Alloc.t_Global &
+            Alloc.Vec.t_Vec u128 Alloc.Alloc.t_Global) =
+            temp_0_
+          in
+          let ll:usize = ll in
+          b2t
+          (((Alloc.Vec.impl_1__len #u128 #Alloc.Alloc.t_Global hi <: usize) =. l <: bool) &&
+            ((Alloc.Vec.impl_1__len #t_Commitment #Alloc.Alloc.t_Global commhi <: usize) =. ll
+              <:
+              bool)) /\
+          b2t
+          ((Alloc.Vec.impl_1__len #Polytune.Data_types.t_Share #Alloc.Alloc.t_Global zshares
+              <:
+              usize) >=.
+            l
+            <:
+            bool) /\
+          (forall (ll: usize).
+              b2t
+              ((mk_usize 0 <=. ll <: bool) && (ll <. l <: bool) &&
+                ((Alloc.Vec.impl_1__len #Polytune.Data_types.t_Share #Alloc.Alloc.t_Global zshares
+                    <:
+                    usize) >=.
+                  l
+                  <:
+                  bool)) ==>
+              b2t
+              ((Alloc.Vec.impl_1__len #(Polytune.Data_types.t_Mac & Polytune.Data_types.t_Key)
+                    #Alloc.Alloc.t_Global
+                    (zshares.[ ll ] <: Polytune.Data_types.t_Share).Polytune.Data_types._1
+                      .Polytune.Data_types._0
+                  <:
+                  usize) >=.
+                n
                 <:
-                Core.Ops.Control_flow.t_ControlFlow
-                  (iimpl_951670863_ &
-                    Core.Result.t_Result
-                      (Alloc.Vec.t_Vec Polytune.Data_types.t_Share Alloc.Alloc.t_Global) t_Error)
-                  (Alloc.Vec.t_Vec (Alloc.Vec.t_Vec u128 Alloc.Alloc.t_Global) Alloc.Alloc.t_Global &
-                    Alloc.Vec.t_Vec Polytune.Data_types.t_Share Alloc.Alloc.t_Global)
-              with
-              | Core.Ops.Control_flow.ControlFlow_Break ret -> ret
-              | Core.Ops.Control_flow.ControlFlow_Continue (ki_xj_phi, zshares) ->
-                let hi:Alloc.Vec.t_Vec u128 Alloc.Alloc.t_Global =
-                  Alloc.Vec.from_elem #u128 (mk_u128 0) l
-                in
-                let commhi:Alloc.Vec.t_Vec t_Commitment Alloc.Alloc.t_Global =
-                  Alloc.Vec.impl__with_capacity #t_Commitment l
-                in
-                let commhi, hi:(Alloc.Vec.t_Vec t_Commitment Alloc.Alloc.t_Global &
-                  Alloc.Vec.t_Vec u128 Alloc.Alloc.t_Global) =
-                  Rust_primitives.Hax.Folds.fold_range (mk_usize 0)
-                    l
-                    (fun temp_0_ temp_1_ ->
-                        let commhi, hi:(Alloc.Vec.t_Vec t_Commitment Alloc.Alloc.t_Global &
-                          Alloc.Vec.t_Vec u128 Alloc.Alloc.t_Global) =
-                          temp_0_
-                        in
-                        let _:usize = temp_1_ in
-                        true)
-                    (commhi, hi
+                bool)))
+      (commhi, hi
+        <:
+        (Alloc.Vec.t_Vec t_Commitment Alloc.Alloc.t_Global &
+          Alloc.Vec.t_Vec u128 Alloc.Alloc.t_Global))
+      (fun temp_0_ ll ->
+          let commhi, hi:(Alloc.Vec.t_Vec t_Commitment Alloc.Alloc.t_Global &
+            Alloc.Vec.t_Vec u128 Alloc.Alloc.t_Global) =
+            temp_0_
+          in
+          let ll:usize = ll in
+          let hi:Alloc.Vec.t_Vec u128 Alloc.Alloc.t_Global =
+            Rust_primitives.Hax.Folds.fold_range (mk_usize 0)
+              n
+              (fun hi temp_1_ ->
+                  let hi:Alloc.Vec.t_Vec u128 Alloc.Alloc.t_Global = hi in
+                  let _:usize = temp_1_ in
+                  b2t
+                  (((Alloc.Vec.impl_1__len #u128 #Alloc.Alloc.t_Global hi <: usize) =. l <: bool) &&
+                    ((Alloc.Vec.impl_1__len #t_Commitment #Alloc.Alloc.t_Global commhi <: usize) =.
+                      ll
                       <:
-                      (Alloc.Vec.t_Vec t_Commitment Alloc.Alloc.t_Global &
-                        Alloc.Vec.t_Vec u128 Alloc.Alloc.t_Global))
-                    (fun temp_0_ ll ->
-                        let commhi, hi:(Alloc.Vec.t_Vec t_Commitment Alloc.Alloc.t_Global &
-                          Alloc.Vec.t_Vec u128 Alloc.Alloc.t_Global) =
-                          temp_0_
-                        in
-                        let ll:usize = ll in
-                        let hi:Alloc.Vec.t_Vec u128 Alloc.Alloc.t_Global =
-                          Rust_primitives.Hax.Folds.fold_range (mk_usize 0)
-                            n
-                            (fun hi temp_1_ ->
-                                let hi:Alloc.Vec.t_Vec u128 Alloc.Alloc.t_Global = hi in
-                                let _:usize = temp_1_ in
-                                true)
-                            hi
-                            (fun hi k ->
-                                let hi:Alloc.Vec.t_Vec u128 Alloc.Alloc.t_Global = hi in
-                                let k:usize = k in
-                                if k =. i <: bool
-                                then hi
-                                else
-                                  let mk_zi, ki_zk:(Polytune.Data_types.t_Mac &
-                                    Polytune.Data_types.t_Key) =
-                                    (zshares.[ ll ] <: Polytune.Data_types.t_Share)
-                                      .Polytune.Data_types._1
-                                      .Polytune.Data_types._0.[ k ]
-                                  in
-                                  Rust_primitives.Hax.Monomorphized_update_at.update_at_usize hi
-                                    ll
-                                    ((((hi.[ ll ] <: u128) ^. mk_zi.Polytune.Data_types._0 <: u128) ^.
-                                        ki_zk.Polytune.Data_types._0
-                                        <:
-                                        u128) ^.
-                                      ((ki_xj_phi.[ k ] <: Alloc.Vec.t_Vec u128 Alloc.Alloc.t_Global
-                                        ).[ ll ]
-                                        <:
-                                        u128)
-                                      <:
-                                      u128))
-                        in
-                        let hi:Alloc.Vec.t_Vec u128 Alloc.Alloc.t_Global =
-                          Rust_primitives.Hax.Monomorphized_update_at.update_at_usize hi
-                            ll
-                            (((hi.[ ll ] <: u128) ^.
-                                ((cast ((xshares.[ ll ] <: Polytune.Data_types.t_Share)
-                                          .Polytune.Data_types._0
-                                        <:
-                                        bool)
-                                    <:
-                                    u128) *!
-                                  (phi.[ ll ] <: u128)
+                      bool)) /\
+                  b2t
+                  ((Alloc.Vec.impl_1__len #Polytune.Data_types.t_Share #Alloc.Alloc.t_Global zshares
+                      <:
+                      usize) >=.
+                    l
+                    <:
+                    bool) /\
+                  (forall (ll: usize).
+                      b2t
+                      ((mk_usize 0 <=. ll <: bool) && (ll <. l <: bool) &&
+                        ((Alloc.Vec.impl_1__len #Polytune.Data_types.t_Share
+                              #Alloc.Alloc.t_Global
+                              zshares
+                            <:
+                            usize) >=.
+                          l
+                          <:
+                          bool)) ==>
+                      b2t
+                      ((Alloc.Vec.impl_1__len #(Polytune.Data_types.t_Mac &
+                              Polytune.Data_types.t_Key)
+                            #Alloc.Alloc.t_Global
+                            (zshares.[ ll ] <: Polytune.Data_types.t_Share).Polytune.Data_types._1
+                              .Polytune.Data_types._0
+                          <:
+                          usize) >=.
+                        n
+                        <:
+                        bool)))
+              hi
+              (fun hi k ->
+                  let hi:Alloc.Vec.t_Vec u128 Alloc.Alloc.t_Global = hi in
+                  let k:usize = k in
+                  if k =. i <: bool
+                  then hi
+                  else
+                    let mk_zi, ki_zk:(Polytune.Data_types.t_Mac & Polytune.Data_types.t_Key) =
+                      (zshares.[ ll ] <: Polytune.Data_types.t_Share).Polytune.Data_types._1
+                        .Polytune.Data_types._0.[ k ]
+                    in
+                    Rust_primitives.Hax.Monomorphized_update_at.update_at_usize hi
+                      ll
+                      ((((hi.[ ll ] <: u128) ^. mk_zi.Polytune.Data_types._0 <: u128) ^.
+                          ki_zk.Polytune.Data_types._0
+                          <:
+                          u128) ^.
+                        ((ki_xj_phi.[ k ] <: Alloc.Vec.t_Vec u128 Alloc.Alloc.t_Global).[ ll ]
+                          <:
+                          u128)
+                        <:
+                        u128))
+          in
+          let hi:Alloc.Vec.t_Vec u128 Alloc.Alloc.t_Global =
+            Rust_primitives.Hax.Monomorphized_update_at.update_at_usize hi
+              ll
+              (((hi.[ ll ] <: u128) ^.
+                  ((cast ((xshares.[ ll ] <: Polytune.Data_types.t_Share).Polytune.Data_types._0
+                          <:
+                          bool)
+                      <:
+                      u128) *!
+                    (phi.[ ll ] <: u128)
+                    <:
+                    u128)
+                  <:
+                  u128) ^.
+                ((cast ((zshares.[ ll ] <: Polytune.Data_types.t_Share).Polytune.Data_types._0
+                        <:
+                        bool)
+                    <:
+                    u128) *!
+                  delta.Polytune.Data_types._0
+                  <:
+                  u128)
+                <:
+                u128)
+          in
+          let commhi:Alloc.Vec.t_Vec t_Commitment Alloc.Alloc.t_Global =
+            Alloc.Vec.impl_1__push #t_Commitment
+              #Alloc.Alloc.t_Global
+              commhi
+              (commit (Core.Num.impl_u128__to_be_bytes (hi.[ ll ] <: u128) <: t_Slice u8)
+                <:
+                t_Commitment)
+          in
+          commhi, hi
+          <:
+          (Alloc.Vec.t_Vec t_Commitment Alloc.Alloc.t_Global &
+            Alloc.Vec.t_Vec u128 Alloc.Alloc.t_Global))
+  in
+  let hax_temp_output:Core.Result.t_Result
+    (Alloc.Vec.t_Vec t_Commitment Alloc.Alloc.t_Global & Alloc.Vec.t_Vec u128 Alloc.Alloc.t_Global)
+    t_Error =
+    Core.Result.Result_Ok
+    (commhi, hi
+      <:
+      (Alloc.Vec.t_Vec t_Commitment Alloc.Alloc.t_Global & Alloc.Vec.t_Vec u128 Alloc.Alloc.t_Global
+      ))
+    <:
+    Core.Result.t_Result
+      (Alloc.Vec.t_Vec t_Commitment Alloc.Alloc.t_Global & Alloc.Vec.t_Vec u128 Alloc.Alloc.t_Global
+      ) t_Error
+  in
+  ki_xj_phi, zshares, hax_temp_output
+  <:
+  (Alloc.Vec.t_Vec (Alloc.Vec.t_Vec u128 Alloc.Alloc.t_Global) Alloc.Alloc.t_Global &
+    Alloc.Vec.t_Vec Polytune.Data_types.t_Share Alloc.Alloc.t_Global &
+    Core.Result.t_Result
+      (Alloc.Vec.t_Vec t_Commitment Alloc.Alloc.t_Global & Alloc.Vec.t_Vec u128 Alloc.Alloc.t_Global
+      ) t_Error)
+
+let flaand_3_
+      (i n l: usize)
+      (xor_all_hi: Alloc.Vec.t_Vec u128 Alloc.Alloc.t_Global)
+      (commhi_k:
+          Alloc.Vec.t_Vec (Alloc.Vec.t_Vec t_Commitment Alloc.Alloc.t_Global) Alloc.Alloc.t_Global)
+      (hi_k_outer: Alloc.Vec.t_Vec (Alloc.Vec.t_Vec u128 Alloc.Alloc.t_Global) Alloc.Alloc.t_Global)
+    : Prims.Pure (Core.Result.t_Result Prims.unit t_Error)
+      (requires
+        b2t ((Alloc.Vec.impl_1__len #u128 #Alloc.Alloc.t_Global xor_all_hi <: usize) =. l <: bool) /\
+        b2t
+        ((Alloc.Vec.impl_1__len #(Alloc.Vec.t_Vec t_Commitment Alloc.Alloc.t_Global)
+              #Alloc.Alloc.t_Global
+              commhi_k
+            <:
+            usize) >=.
+          n
+          <:
+          bool) /\
+        (forall (k: usize).
+            b2t
+            ((mk_usize 0 <=. k <: bool) && (k <. n <: bool) &&
+              ((Alloc.Vec.impl_1__len #(Alloc.Vec.t_Vec t_Commitment Alloc.Alloc.t_Global)
+                    #Alloc.Alloc.t_Global
+                    commhi_k
+                  <:
+                  usize) >=.
+                n
+                <:
+                bool)) ==>
+            b2t
+            ((Alloc.Vec.impl_1__len #t_Commitment
+                  #Alloc.Alloc.t_Global
+                  (commhi_k.[ k ] <: Alloc.Vec.t_Vec t_Commitment Alloc.Alloc.t_Global)
+                <:
+                usize) >=.
+              l
+              <:
+              bool)) /\
+        (b2t
+        ((Alloc.Vec.impl_1__len #(Alloc.Vec.t_Vec u128 Alloc.Alloc.t_Global)
+              #Alloc.Alloc.t_Global
+              hi_k_outer
+            <:
+            usize) >=.
+          n
+          <:
+          bool) /\
+        (forall (k: usize).
+            b2t
+            ((mk_usize 0 <=. k <: bool) && (k <. n <: bool) &&
+              ((Alloc.Vec.impl_1__len #(Alloc.Vec.t_Vec u128 Alloc.Alloc.t_Global)
+                    #Alloc.Alloc.t_Global
+                    hi_k_outer
+                  <:
+                  usize) >=.
+                n
+                <:
+                bool)) ==>
+            b2t
+            ((Alloc.Vec.impl_1__len #u128
+                  #Alloc.Alloc.t_Global
+                  (hi_k_outer.[ k ] <: Alloc.Vec.t_Vec u128 Alloc.Alloc.t_Global)
+                <:
+                usize) >=.
+              l
+              <:
+              bool))))
+      (fun _ -> Prims.l_True) =
+  let commitment_error:bool = false in
+  let xor_not_zero_error:bool = false in
+  let commitment_error, xor_all_hi:(bool & Alloc.Vec.t_Vec u128 Alloc.Alloc.t_Global) =
+    Rust_primitives.Hax.Folds.fold_range (mk_usize 0)
+      n
+      (fun temp_0_ temp_1_ ->
+          let commitment_error, xor_all_hi:(bool & Alloc.Vec.t_Vec u128 Alloc.Alloc.t_Global) =
+            temp_0_
+          in
+          let _:usize = temp_1_ in
+          (Alloc.Vec.impl_1__len #u128 #Alloc.Alloc.t_Global xor_all_hi <: usize) =. l <: bool)
+      (commitment_error, xor_all_hi <: (bool & Alloc.Vec.t_Vec u128 Alloc.Alloc.t_Global))
+      (fun temp_0_ k ->
+          let commitment_error, xor_all_hi:(bool & Alloc.Vec.t_Vec u128 Alloc.Alloc.t_Global) =
+            temp_0_
+          in
+          let k:usize = k in
+          if k =. i <: bool
+          then commitment_error, xor_all_hi <: (bool & Alloc.Vec.t_Vec u128 Alloc.Alloc.t_Global)
+          else
+            Rust_primitives.Hax.Folds.fold_range (mk_usize 0)
+              l
+              (fun temp_0_ temp_1_ ->
+                  let commitment_error, xor_all_hi:(bool & Alloc.Vec.t_Vec u128 Alloc.Alloc.t_Global
+                  ) =
+                    temp_0_
+                  in
+                  let _:usize = temp_1_ in
+                  (Alloc.Vec.impl_1__len #u128 #Alloc.Alloc.t_Global xor_all_hi <: usize) =. l
+                  <:
+                  bool)
+              (commitment_error, xor_all_hi <: (bool & Alloc.Vec.t_Vec u128 Alloc.Alloc.t_Global))
+              (fun temp_0_ ll ->
+                  let commitment_error, xor_all_hi:(bool & Alloc.Vec.t_Vec u128 Alloc.Alloc.t_Global
+                  ) =
+                    temp_0_
+                  in
+                  let ll:usize = ll in
+                  let commitment_error:bool =
+                    if
+                      ~.(open_commitment ((commhi_k.[ k ]
+                              <:
+                              Alloc.Vec.t_Vec t_Commitment Alloc.Alloc.t_Global).[ ll ]
+                            <:
+                            t_Commitment)
+                          (Core.Num.impl_u128__to_be_bytes ((hi_k_outer.[ k ]
                                   <:
-                                  u128)
-                                <:
-                                u128) ^.
-                              ((cast ((zshares.[ ll ] <: Polytune.Data_types.t_Share)
-                                        .Polytune.Data_types._0
-                                      <:
-                                      bool)
-                                  <:
-                                  u128) *!
-                                delta.Polytune.Data_types._0
+                                  Alloc.Vec.t_Vec u128 Alloc.Alloc.t_Global).[ ll ]
                                 <:
                                 u128)
-                              <:
-                              u128)
-                        in
-                        let commhi:Alloc.Vec.t_Vec t_Commitment Alloc.Alloc.t_Global =
-                          Alloc.Vec.impl_1__push #t_Commitment
-                            #Alloc.Alloc.t_Global
-                            commhi
-                            (commit (Core.Num.impl_u128__to_be_bytes (hi.[ ll ] <: u128)
-                                  <:
-                                  t_Slice u8)
-                              <:
-                              t_Commitment)
-                        in
-                        commhi, hi
+                            <:
+                            t_Slice u8)
                         <:
-                        (Alloc.Vec.t_Vec t_Commitment Alloc.Alloc.t_Global &
-                          Alloc.Vec.t_Vec u128 Alloc.Alloc.t_Global))
-                in
-                let tmp0, out:(iimpl_951670863_ &
-                  Core.Result.t_Result
-                    (Alloc.Vec.t_Vec (Alloc.Vec.t_Vec t_Commitment Alloc.Alloc.t_Global)
-                        Alloc.Alloc.t_Global) t_Error) =
-                  broadcast #t_Commitment
-                    #iimpl_951670863_
-                    channel
-                    i
-                    n
-                    "flaand comm"
-                    (Core.Ops.Deref.f_deref #(Alloc.Vec.t_Vec t_Commitment Alloc.Alloc.t_Global)
-                        #FStar.Tactics.Typeclasses.solve
-                        commhi
-                      <:
-                      t_Slice t_Commitment)
-                    l
-                in
-                let channel:iimpl_951670863_ = tmp0 in
-                match
-                  out
-                  <:
-                  Core.Result.t_Result
-                    (Alloc.Vec.t_Vec (Alloc.Vec.t_Vec t_Commitment Alloc.Alloc.t_Global)
-                        Alloc.Alloc.t_Global) t_Error
-                with
-                | Core.Result.Result_Ok commhi_k ->
-                  let tmp0, out:(iimpl_951670863_ &
-                    Core.Result.t_Result
-                      (Alloc.Vec.t_Vec (Alloc.Vec.t_Vec u128 Alloc.Alloc.t_Global)
-                          Alloc.Alloc.t_Global) t_Error) =
-                    broadcast #u128
-                      #iimpl_951670863_
-                      channel
-                      i
-                      n
-                      "flaand hash"
-                      (Core.Ops.Deref.f_deref #(Alloc.Vec.t_Vec u128 Alloc.Alloc.t_Global)
-                          #FStar.Tactics.Typeclasses.solve
-                          hi
-                        <:
-                        t_Slice u128)
-                      l
+                        bool)
+                    then
+                      let commitment_error:bool = true in
+                      commitment_error
+                    else commitment_error
                   in
-                  let channel:iimpl_951670863_ = tmp0 in
-                  (match
-                      out
-                      <:
-                      Core.Result.t_Result
-                        (Alloc.Vec.t_Vec (Alloc.Vec.t_Vec u128 Alloc.Alloc.t_Global)
-                            Alloc.Alloc.t_Global) t_Error
-                    with
-                    | Core.Result.Result_Ok hi_k_outer ->
-                      let xor_all_hi:Alloc.Vec.t_Vec u128 Alloc.Alloc.t_Global = hi in
-                      (match
-                          Rust_primitives.Hax.Folds.fold_range_return (mk_usize 0)
-                            n
-                            (fun xor_all_hi temp_1_ ->
-                                let xor_all_hi:Alloc.Vec.t_Vec u128 Alloc.Alloc.t_Global =
-                                  xor_all_hi
-                                in
-                                let _:usize = temp_1_ in
-                                true)
-                            xor_all_hi
-                            (fun xor_all_hi k ->
-                                let xor_all_hi:Alloc.Vec.t_Vec u128 Alloc.Alloc.t_Global =
-                                  xor_all_hi
-                                in
-                                let k:usize = k in
-                                if k =. i <: bool
-                                then
-                                  Core.Ops.Control_flow.ControlFlow_Continue xor_all_hi
-                                  <:
-                                  Core.Ops.Control_flow.t_ControlFlow
-                                    (Core.Ops.Control_flow.t_ControlFlow
-                                        (iimpl_951670863_ &
-                                          Core.Result.t_Result
-                                            (Alloc.Vec.t_Vec Polytune.Data_types.t_Share
-                                                Alloc.Alloc.t_Global) t_Error)
-                                        (Prims.unit & Alloc.Vec.t_Vec u128 Alloc.Alloc.t_Global))
-                                    (Alloc.Vec.t_Vec u128 Alloc.Alloc.t_Global)
-                                else
-                                  match
-                                    Rust_primitives.Hax.Folds.fold_range_return (mk_usize 0)
-                                      (Alloc.Vec.impl_1__len #u128 #Alloc.Alloc.t_Global xor_all_hi
-                                        <:
-                                        usize)
-                                      (fun xor_all_hi temp_1_ ->
-                                          let xor_all_hi:Alloc.Vec.t_Vec u128 Alloc.Alloc.t_Global =
-                                            xor_all_hi
-                                          in
-                                          let _:usize = temp_1_ in
-                                          true)
-                                      xor_all_hi
-                                      (fun xor_all_hi ll ->
-                                          let xor_all_hi:Alloc.Vec.t_Vec u128 Alloc.Alloc.t_Global =
-                                            xor_all_hi
-                                          in
-                                          let ll:usize = ll in
-                                          if
-                                            ~.(open_commitment ((commhi_k.[ k ]
-                                                    <:
-                                                    Alloc.Vec.t_Vec t_Commitment
-                                                      Alloc.Alloc.t_Global).[ ll ]
-                                                  <:
-                                                  t_Commitment)
-                                                (Core.Num.impl_u128__to_be_bytes ((hi_k_outer.[ k ]
-                                                        <:
-                                                        Alloc.Vec.t_Vec u128 Alloc.Alloc.t_Global).[
-                                                        ll ]
-                                                      <:
-                                                      u128)
-                                                  <:
-                                                  t_Slice u8)
-                                              <:
-                                              bool)
-                                            <:
-                                            bool
-                                          then
-                                            Core.Ops.Control_flow.ControlFlow_Break
-                                            (Core.Ops.Control_flow.ControlFlow_Break
-                                              (channel,
-                                                (Core.Result.Result_Err
-                                                  (Error_CommitmentCouldNotBeOpened <: t_Error)
-                                                  <:
-                                                  Core.Result.t_Result
-                                                    (Alloc.Vec.t_Vec Polytune.Data_types.t_Share
-                                                        Alloc.Alloc.t_Global) t_Error)
-                                                <:
-                                                (iimpl_951670863_ &
-                                                  Core.Result.t_Result
-                                                    (Alloc.Vec.t_Vec Polytune.Data_types.t_Share
-                                                        Alloc.Alloc.t_Global) t_Error))
-                                              <:
-                                              Core.Ops.Control_flow.t_ControlFlow
-                                                (iimpl_951670863_ &
-                                                  Core.Result.t_Result
-                                                    (Alloc.Vec.t_Vec Polytune.Data_types.t_Share
-                                                        Alloc.Alloc.t_Global) t_Error)
-                                                (Prims.unit &
-                                                  Alloc.Vec.t_Vec u128 Alloc.Alloc.t_Global))
-                                            <:
-                                            Core.Ops.Control_flow.t_ControlFlow
-                                              (Core.Ops.Control_flow.t_ControlFlow
-                                                  (iimpl_951670863_ &
-                                                    Core.Result.t_Result
-                                                      (Alloc.Vec.t_Vec Polytune.Data_types.t_Share
-                                                          Alloc.Alloc.t_Global) t_Error)
-                                                  (Prims.unit &
-                                                    Alloc.Vec.t_Vec u128 Alloc.Alloc.t_Global))
-                                              (Alloc.Vec.t_Vec u128 Alloc.Alloc.t_Global)
-                                          else
-                                            Core.Ops.Control_flow.ControlFlow_Continue
-                                            (Rust_primitives.Hax.Monomorphized_update_at.update_at_usize
-                                                xor_all_hi
-                                                ll
-                                                ((xor_all_hi.[ ll ] <: u128) ^.
-                                                  ((hi_k_outer.[ k ]
-                                                      <:
-                                                      Alloc.Vec.t_Vec u128 Alloc.Alloc.t_Global).[ ll
-                                                    ]
-                                                    <:
-                                                    u128)
-                                                  <:
-                                                  u128)
-                                              <:
-                                              Alloc.Vec.t_Vec u128 Alloc.Alloc.t_Global)
-                                            <:
-                                            Core.Ops.Control_flow.t_ControlFlow
-                                              (Core.Ops.Control_flow.t_ControlFlow
-                                                  (iimpl_951670863_ &
-                                                    Core.Result.t_Result
-                                                      (Alloc.Vec.t_Vec Polytune.Data_types.t_Share
-                                                          Alloc.Alloc.t_Global) t_Error)
-                                                  (Prims.unit &
-                                                    Alloc.Vec.t_Vec u128 Alloc.Alloc.t_Global))
-                                              (Alloc.Vec.t_Vec u128 Alloc.Alloc.t_Global))
-                                    <:
-                                    Core.Ops.Control_flow.t_ControlFlow
-                                      (iimpl_951670863_ &
-                                        Core.Result.t_Result
-                                          (Alloc.Vec.t_Vec Polytune.Data_types.t_Share
-                                              Alloc.Alloc.t_Global) t_Error)
-                                      (Alloc.Vec.t_Vec u128 Alloc.Alloc.t_Global)
-                                  with
-                                  | Core.Ops.Control_flow.ControlFlow_Break ret ->
-                                    Core.Ops.Control_flow.ControlFlow_Break
-                                    (Core.Ops.Control_flow.ControlFlow_Break ret
-                                      <:
-                                      Core.Ops.Control_flow.t_ControlFlow
-                                        (iimpl_951670863_ &
-                                          Core.Result.t_Result
-                                            (Alloc.Vec.t_Vec Polytune.Data_types.t_Share
-                                                Alloc.Alloc.t_Global) t_Error)
-                                        (Prims.unit & Alloc.Vec.t_Vec u128 Alloc.Alloc.t_Global))
-                                    <:
-                                    Core.Ops.Control_flow.t_ControlFlow
-                                      (Core.Ops.Control_flow.t_ControlFlow
-                                          (iimpl_951670863_ &
-                                            Core.Result.t_Result
-                                              (Alloc.Vec.t_Vec Polytune.Data_types.t_Share
-                                                  Alloc.Alloc.t_Global) t_Error)
-                                          (Prims.unit & Alloc.Vec.t_Vec u128 Alloc.Alloc.t_Global))
-                                      (Alloc.Vec.t_Vec u128 Alloc.Alloc.t_Global)
-                                  | Core.Ops.Control_flow.ControlFlow_Continue loop_res ->
-                                    Core.Ops.Control_flow.ControlFlow_Continue loop_res
-                                    <:
-                                    Core.Ops.Control_flow.t_ControlFlow
-                                      (Core.Ops.Control_flow.t_ControlFlow
-                                          (iimpl_951670863_ &
-                                            Core.Result.t_Result
-                                              (Alloc.Vec.t_Vec Polytune.Data_types.t_Share
-                                                  Alloc.Alloc.t_Global) t_Error)
-                                          (Prims.unit & Alloc.Vec.t_Vec u128 Alloc.Alloc.t_Global))
-                                      (Alloc.Vec.t_Vec u128 Alloc.Alloc.t_Global))
+                  let xor_all_hi:Alloc.Vec.t_Vec u128 Alloc.Alloc.t_Global =
+                    Rust_primitives.Hax.Monomorphized_update_at.update_at_usize xor_all_hi
+                      ll
+                      ((xor_all_hi.[ ll ] <: u128) ^.
+                        ((hi_k_outer.[ k ] <: Alloc.Vec.t_Vec u128 Alloc.Alloc.t_Global).[ ll ]
                           <:
-                          Core.Ops.Control_flow.t_ControlFlow
-                            (iimpl_951670863_ &
-                              Core.Result.t_Result
-                                (Alloc.Vec.t_Vec Polytune.Data_types.t_Share Alloc.Alloc.t_Global)
-                                t_Error) (Alloc.Vec.t_Vec u128 Alloc.Alloc.t_Global)
-                        with
-                        | Core.Ops.Control_flow.ControlFlow_Break ret -> ret
-                        | Core.Ops.Control_flow.ControlFlow_Continue xor_all_hi ->
-                          match
-                            Rust_primitives.Hax.Folds.fold_range_return (mk_usize 0)
-                              l
-                              (fun temp_0_ temp_1_ ->
-                                  let _:Prims.unit = temp_0_ in
-                                  let _:usize = temp_1_ in
-                                  true)
-                              ()
-                              (fun temp_0_ i ->
-                                  let _:Prims.unit = temp_0_ in
-                                  let i:usize = i in
-                                  if (xor_all_hi.[ i ] <: u128) <>. mk_u128 0 <: bool
-                                  then
-                                    Core.Ops.Control_flow.ControlFlow_Break
-                                    (Core.Ops.Control_flow.ControlFlow_Break
-                                      (channel,
-                                        (Core.Result.Result_Err (Error_LaANDXorNotZero <: t_Error)
-                                          <:
-                                          Core.Result.t_Result
-                                            (Alloc.Vec.t_Vec Polytune.Data_types.t_Share
-                                                Alloc.Alloc.t_Global) t_Error)
-                                        <:
-                                        (iimpl_951670863_ &
-                                          Core.Result.t_Result
-                                            (Alloc.Vec.t_Vec Polytune.Data_types.t_Share
-                                                Alloc.Alloc.t_Global) t_Error))
-                                      <:
-                                      Core.Ops.Control_flow.t_ControlFlow
-                                        (iimpl_951670863_ &
-                                          Core.Result.t_Result
-                                            (Alloc.Vec.t_Vec Polytune.Data_types.t_Share
-                                                Alloc.Alloc.t_Global) t_Error)
-                                        (Prims.unit & Prims.unit))
-                                    <:
-                                    Core.Ops.Control_flow.t_ControlFlow
-                                      (Core.Ops.Control_flow.t_ControlFlow
-                                          (iimpl_951670863_ &
-                                            Core.Result.t_Result
-                                              (Alloc.Vec.t_Vec Polytune.Data_types.t_Share
-                                                  Alloc.Alloc.t_Global) t_Error)
-                                          (Prims.unit & Prims.unit)) Prims.unit
-                                  else
-                                    Core.Ops.Control_flow.ControlFlow_Continue ()
-                                    <:
-                                    Core.Ops.Control_flow.t_ControlFlow
-                                      (Core.Ops.Control_flow.t_ControlFlow
-                                          (iimpl_951670863_ &
-                                            Core.Result.t_Result
-                                              (Alloc.Vec.t_Vec Polytune.Data_types.t_Share
-                                                  Alloc.Alloc.t_Global) t_Error)
-                                          (Prims.unit & Prims.unit)) Prims.unit)
-                            <:
-                            Core.Ops.Control_flow.t_ControlFlow
-                              (iimpl_951670863_ &
-                                Core.Result.t_Result
-                                  (Alloc.Vec.t_Vec Polytune.Data_types.t_Share Alloc.Alloc.t_Global)
-                                  t_Error) Prims.unit
-                          with
-                          | Core.Ops.Control_flow.ControlFlow_Break ret -> ret
-                          | Core.Ops.Control_flow.ControlFlow_Continue _ ->
-                            let hax_temp_output:Core.Result.t_Result
-                              (Alloc.Vec.t_Vec Polytune.Data_types.t_Share Alloc.Alloc.t_Global)
-                              t_Error =
-                              Core.Result.Result_Ok zshares
-                              <:
-                              Core.Result.t_Result
-                                (Alloc.Vec.t_Vec Polytune.Data_types.t_Share Alloc.Alloc.t_Global)
-                                t_Error
-                            in
-                            channel, hax_temp_output
-                            <:
-                            (iimpl_951670863_ &
-                              Core.Result.t_Result
-                                (Alloc.Vec.t_Vec Polytune.Data_types.t_Share Alloc.Alloc.t_Global)
-                                t_Error))
-                    | Core.Result.Result_Err err ->
-                      channel,
-                      (Core.Result.Result_Err err
+                          u128)
                         <:
-                        Core.Result.t_Result
-                          (Alloc.Vec.t_Vec Polytune.Data_types.t_Share Alloc.Alloc.t_Global) t_Error
-                      )
-                      <:
-                      (iimpl_951670863_ &
-                        Core.Result.t_Result
-                          (Alloc.Vec.t_Vec Polytune.Data_types.t_Share Alloc.Alloc.t_Global) t_Error
-                      ))
-                | Core.Result.Result_Err err ->
-                  channel,
-                  (Core.Result.Result_Err err
-                    <:
-                    Core.Result.t_Result
-                      (Alloc.Vec.t_Vec Polytune.Data_types.t_Share Alloc.Alloc.t_Global) t_Error)
-                  <:
-                  (iimpl_951670863_ &
-                    Core.Result.t_Result
-                      (Alloc.Vec.t_Vec Polytune.Data_types.t_Share Alloc.Alloc.t_Global) t_Error))
-          | Core.Result.Result_Err err ->
-            channel,
-            (Core.Result.Result_Err err
-              <:
-              Core.Result.t_Result
-                (Alloc.Vec.t_Vec Polytune.Data_types.t_Share Alloc.Alloc.t_Global) t_Error)
+                        u128)
+                  in
+                  commitment_error, xor_all_hi <: (bool & Alloc.Vec.t_Vec u128 Alloc.Alloc.t_Global)
+              )
             <:
-            (iimpl_951670863_ &
-              Core.Result.t_Result
-                (Alloc.Vec.t_Vec Polytune.Data_types.t_Share Alloc.Alloc.t_Global) t_Error))
-    | Core.Result.Result_Err err ->
-      channel,
-      (Core.Result.Result_Err err
-        <:
-        Core.Result.t_Result (Alloc.Vec.t_Vec Polytune.Data_types.t_Share Alloc.Alloc.t_Global)
-          t_Error)
+            (bool & Alloc.Vec.t_Vec u128 Alloc.Alloc.t_Global))
+  in
+  let xor_not_zero_error:bool =
+    Rust_primitives.Hax.Folds.fold_range (mk_usize 0)
+      l
+      (fun xor_not_zero_error temp_1_ ->
+          let xor_not_zero_error:bool = xor_not_zero_error in
+          let _:usize = temp_1_ in
+          (Alloc.Vec.impl_1__len #u128 #Alloc.Alloc.t_Global xor_all_hi <: usize) =. l <: bool)
+      xor_not_zero_error
+      (fun xor_not_zero_error i ->
+          let xor_not_zero_error:bool = xor_not_zero_error in
+          let i:usize = i in
+          if (xor_all_hi.[ i ] <: u128) <>. mk_u128 0 <: bool
+          then
+            let xor_not_zero_error:bool = true in
+            xor_not_zero_error
+          else xor_not_zero_error)
+  in
+  if commitment_error
+  then
+    Core.Result.Result_Err (Error_CommitmentCouldNotBeOpened <: t_Error)
+    <:
+    Core.Result.t_Result Prims.unit t_Error
+  else
+    if xor_not_zero_error
+    then
+      Core.Result.Result_Err (Error_LaANDXorNotZero <: t_Error)
       <:
-      (iimpl_951670863_ &
-        Core.Result.t_Result (Alloc.Vec.t_Vec Polytune.Data_types.t_Share Alloc.Alloc.t_Global)
-          t_Error)
+      Core.Result.t_Result Prims.unit t_Error
+    else Core.Result.Result_Ok (() <: Prims.unit) <: Core.Result.t_Result Prims.unit t_Error
